Blanc/ReSemantics.lean
@@ -1,0 +1,2408 @@
+-- Semantics.lean : formalized semantics of the EVM and Blanc
+
+import Blanc.Basic
+import Elevm.Hash
+import Elevm.Execution
+
+
+
+def Rinst.toB8 : Rinst → B8
+  | add          => 0x01
+  | mul          => 0x02
+  | sub          => 0x03
+  | div          => 0x04
+  | sdiv         => 0x05
+  | mod          => 0x06
+  | smod         => 0x07
+  | addmod       => 0x08
+  | mulmod       => 0x09
+  | exp          => 0x0A
+  | signextend   => 0x0B
+  | lt           => 0x10
+  | gt           => 0x11
+  | slt          => 0x12
+  | sgt          => 0x13
+  | eq           => 0x14
+  | iszero       => 0x15
+  | and          => 0x16
+  | or           => 0x17
+  | xor          => 0x18
+  | not          => 0x19
+  | byte         => 0x1A
+  | shl          => 0x1B
+  | shr          => 0x1C
+  | sar          => 0x1D
+  | kec          => 0x20
+  | address      => 0x30
+  | balance      => 0x31
+  | origin       => 0x32
+  | caller       => 0x33
+  | callvalue    => 0x34
+  | calldataload => 0x35
+  | calldatasize => 0x36
+  | calldatacopy => 0x37
+  | codesize     => 0x38
+  | codecopy     => 0x39
+  | gasprice     => 0x3A
+  | extcodesize  => 0x3B
+  | extcodecopy  => 0x3C
+  | retdatasize  => 0x3D
+  | retdatacopy  => 0x3E
+  | extcodehash  => 0x3F
+  | blockhash    => 0x40
+  | coinbase     => 0x41
+  | timestamp    => 0x42
+  | number       => 0x43
+  | prevrandao   => 0x44
+  | gaslimit     => 0x45
+  | chainid      => 0x46
+  | selfbalance  => 0x47
+  | basefee      => 0x48
+  | blobhash     => 0x49
+  | blobbasefee  => 0x4A
+  | pop          => 0x50
+  | mload        => 0x51
+  | mstore       => 0x52
+  | mstore8      => 0x53
+  | sload        => 0x54
+  | sstore       => 0x55
+  | pc           => 0x58
+  | msize        => 0x59
+  | gas          => 0x5A
+  | tload        => 0x5C
+  | tstore       => 0x5D
+  | mcopy        => 0x5E
+  | dup n        => 0x80 + n.val.toUInt8
+  | swap n       => 0x90 + n.val.toUInt8
+  | log n        => 0xA0 + n.val.toUInt8
+
+abbrev Stack : Type := List B256
+
+def Stack.Push (x y xy : Stack) : Prop := x <++ xy ++> y
+def Stack.Pop (x xy y : Stack) : Prop := x <++ xy ++> y
+def Stack.Diff (xs zs : Stack) (s s'' : Stack) : Prop :=
+  ∃ s' : Stack, Pop xs s s' ∧ Push zs s' s''
+
+inductive Func : Type
+  | branch : Func → Func → Func
+  | last : Linst → Func
+  | next : Ninst → Func → Func
+  | call : Nat → Func
+
+structure Prog : Type where
+  (main : Func)
+  (aux : List Func)
+
+def Jinst.Run (evm : Evm) :
+    Jinst → Except (String × Devm) (Nat × Devm) → Prop :=
+  λ j ex => j.run evm = ex
+
+def Linst.Run (sevm : Sevm) (devm : Devm) : Linst → Execution → Prop :=
+  λ l ex => l.run sevm devm = ex
+
+def Xlot : Type := Option (Evm × Execution)
+
+structure Devm.Rels : Type where
+  (stack : List B256 → List B256 → Prop)
+  (memory : Mem → Mem → Prop)
+  (gasLeft : Nat → Nat → Prop)
+  (logs : List Log → List Log → Prop)
+  (refundCounter : Int → Int → Prop)
+  (output : B8L → B8L → Prop)
+  (accountsToDelete : AdrSet → AdrSet → Prop)
+  (returnData : B8L → B8L → Prop)
+  (error : Option String → Option String → Prop)
+  (accessedAddresses : AdrSet → AdrSet → Prop)
+  (accessedStorageKeys : KeySet → KeySet → Prop)
+  (state : State → State → Prop)
+  (createdAccounts : AdrSet → AdrSet → Prop)
+  (transientStorage : Tra → Tra → Prop)
+
+structure Devm.Rel (rels : Devm.Rels) (devm devm' : Devm) : Prop where
+  (stack : rels.stack devm.stack devm'.stack)
+  (memory : rels.memory devm.memory devm'.memory)
+  (gasLeft : rels.gasLeft devm.gasLeft devm'.gasLeft)
+  (logs : rels.logs devm.logs devm'.logs)
+  (refundCounter : rels.refundCounter devm.refundCounter devm'.refundCounter)
+  (output : rels.output devm.output devm'.output)
+  ( accountsToDelete :
+    rels.accountsToDelete devm.accountsToDelete devm'.accountsToDelete)
+  (returnData : rels.returnData devm.returnData devm'.returnData)
+  (error : rels.error devm.error devm'.error)
+  ( accessedAddresses :
+    rels.accessedAddresses devm.accessedAddresses devm'.accessedAddresses )
+  ( accessedStorageKeys :
+    rels.accessedStorageKeys devm.accessedStorageKeys devm'.accessedStorageKeys )
+  (state : rels.state devm.state devm'.state)
+  ( transientStorage :
+    rels.transientStorage devm.transientStorage devm'.transientStorage )
+
+def Devm.Rels.eq : Devm.Rels :=
+  {
+    stack := _root_.Eq,
+    memory := _root_.Eq,
+    gasLeft := _root_.Eq,
+    logs := _root_.Eq,
+    refundCounter := _root_.Eq,
+    output := _root_.Eq,
+    accountsToDelete := _root_.Eq,
+    returnData := _root_.Eq,
+    error := _root_.Eq,
+    accessedAddresses := _root_.Eq,
+    accessedStorageKeys := _root_.Eq,
+    state := _root_.Eq,
+    createdAccounts := _root_.Eq,
+    transientStorage := _root_.Eq
+  }
+
+def Devm.Burn : Devm → Devm → Prop :=
+  Rel {
+    Rels.eq with
+    gasLeft :=
+      λ gas gas' => ∃ diff : Nat, gas = gas' + diff
+  }
+
+def Devm.PopBurn (xs : List B256) : Devm → Devm → Prop :=
+  Rel {
+    Rels.eq with
+    stack := Stack.Pop xs
+    gasLeft :=
+      λ gas gas' => ∃ diff : Nat, gas = gas' + diff
+  }
+
+def Linst.At (code : ByteArray) (pc : Nat) (l : Linst) : Prop := code.getInst pc = some (.last l)
+def Ninst.At (code : ByteArray) (pc : Nat) (n : Ninst) : Prop := code.getInst pc = some (.next n)
+def Jinst.At (code : ByteArray) (pc : Nat) (j : Jinst) : Prop := code.getInst pc = some (.jump j)
+def Rinst.At (code : ByteArray) (pc : Nat) (r : Rinst) : Prop := code.getInst pc = some (.next (.reg r))
+
+def Execution.withPc (pc : Nat) (exn : Execution) :
+     Except (String × Devm) (Nat × Devm) := do
+  let devm ← exn
+  .ok ⟨pc, devm⟩
+
+def Except.Split {ξ υ ζ : Type}
+    (e : Except ξ υ) (e' : Except ξ ζ) (q : υ → Prop) : Prop :=
+  (∃ x, e = .error x ∧ e' = .error x) ∨ (∃ y : υ, e = .ok y ∧ q y)
+
+def ExecuteCode (msg : Msg) (xl : Xlot)
+    (ex : Except (String × State × AdrSet × Tra) Devm) : Prop :=
+  let evm : Evm := initEvm msg
+  match msg.codeAddress with
+  | .none =>
+    ∃ ex', xl = .some ⟨evm, ex'⟩ ∧ executeCode.handleError ex' = ex
+  | .some adr =>
+    if adr.isPrecomp then
+      (xl = .none ∧  executeCode.handleError (executePrecomp evm adr) = ex)
+    else
+      ∃ ex', xl = .some ⟨evm, ex'⟩ ∧ executeCode.handleError ex' = ex
+
+def ProcessMessage (msg : Msg) (xl : Xlot)
+    (ex : Except (String × State × AdrSet × Tra) Devm) : Prop :=
+    ( Except.assert (msg.depth ≤ 1024)
+        ⟨ "StackDepthLimitError",
+          msg.benv.state,
+          msg.benv.createdAccounts,
+          msg.tenv.transientStorage ⟩ ).Split ex <|
+  λ _ =>
+    msg.benvAfterTransfer.Split ex <|
+  λ benv =>
+  ∃ ex' : Except (String × State × AdrSet × Tra) Devm,
+    And (ExecuteCode (msg.withBenv benv) xl ex') <|
+    ex'.Split ex <|
+  λ evm =>
+    if evm.error.isSome then
+      .ok (evm.rollback msg.benv.state msg.tenv.transientStorage) = ex
+    else
+      .ok evm = ex
+
+def ProcessCreateMessage (msg : Msg) (xl : Xlot)
+    (ex : Except (String × State × AdrSet × Tra) Devm) : Prop :=
+  ∃ ex' : Except (String × State × AdrSet × Tra) Devm,
+    And (ProcessMessage (processCreateMessage.msg msg) xl ex') <|
+    ex'.Split ex <|
+  λ evm =>
+  if evm.error.isNone then
+    match processCreateMessage.chargeCodeGas evm with
+    | .ok evm => .ok (evm.setCode msg.currentTarget ⟨⟨evm.output⟩⟩) = ex
+    | .error (err, evm) =>
+      if isExceptionalHalt err then
+        .ok
+          ( processCreateMessage.exceptionalHalt evm err
+              msg.benv.state
+              msg.tenv.transientStorage ) = ex
+      else
+        .error ⟨err, evm.state, evm.createdAccounts, evm.transientStorage⟩ = ex
+  else
+    .ok (evm.rollback msg.benv.state msg.tenv.transientStorage) = ex
+
+def ExistsEq {ξ} (t : ξ) (p : ξ → Prop) : Prop :=
+  ∃ x : ξ, (x = t) ∧ p x
+
+def GenericCreate (sevm : Sevm) (devm : Devm) (endowment : B256) (newAddress : Adr)
+    (memoryIndex memorySize : Nat) (xl : Xlot) (ex : Execution) : Prop :=
+    ExistsEq (devm.memory.data.sliceD memoryIndex memorySize 0) <|
+  λ calldata =>
+    ( Except.assert
+        (memorySize ≤ maxInitcodeSize)
+        ⟨"OutOfGasError", devm⟩ ).Split ex <|
+  λ _ =>
+    ExistsEq (addAccessedAddress devm newAddress) <|
+  λ devm1 =>
+    ExistsEq (except64th devm1.gasLeft) <|
+  λ createMsgGas =>
+    ExistsEq ({devm1 with gasLeft := devm1.gasLeft - createMsgGas}) <|
+  λ devm2 =>
+    (assertDynamic sevm devm2).Split ex <|
+  λ _ =>
+    ExistsEq ({devm2 with returnData := []}) <|
+  λ devm3 =>
+    ExistsEq (devm3.state.get sevm.currentTarget) <|
+  λ sender =>
+   if (sender.bal < endowment ∨ sender.nonce = B64.max ∨ sevm.depth + 1 > 1024) then
+     ({devm3 with gasLeft := devm3.gasLeft + createMsgGas}.push 0 = ex)
+   else
+   ExistsEq (devm3.incrNonce sevm.currentTarget) <|
+  λ devm4 =>
+    if
+      ( let target := devm4.state.get newAddress
+        target.nonce ≠ (0 : B64) ∨ target.code.size ≠ 0 ∨ target.stor.size ≠ 0 ) then
+      (devm4.push 0 = ex)
+    else
+    ExistsEq
+      {
+        benv := Benv.mk devm4.state devm4.createdAccounts sevm.benvStat
+        tenv := {transientStorage := devm4.transientStorage, stat := sevm.tenvStat}
+        caller := sevm.currentTarget
+        target := .none
+        gas := createMsgGas
+        value := endowment
+        data := []
+        code := .mk <| .mk calldata
+        currentTarget := newAddress
+        depth := sevm.depth + 1
+        codeAddress := .none
+        shouldTransferValue := true
+        isStatic := false
+        accessedAddresses := devm4.accessedAddresses
+        accessedStorageKeys := devm4.accessedStorageKeys
+        disablePrecompiles := false
+      } <|
+  λ childMsg =>
+  ∃ ex',
+    And (ProcessCreateMessage childMsg xl ex') <|
+    (liftToExecution devm4 ex').Split ex <|
+  λ child =>
+    if child.error.isSome then
+      (incorporateChildOnError devm4 child child.output).push 0 = ex
+    else
+      (incorporateChildOnSuccess devm4 child []).push newAddress.toB256 = ex
+
+def GenericCall
+    (sevm: Sevm)
+    (devm: Devm)
+    (gas: Nat)
+    (value: B256)
+    (caller: Adr)
+    (target: Adr)
+    (codeAddress: Adr)
+    (shouldTransferValue: Bool)
+    (isStaticcall: Bool)
+    (input_index:  Nat)
+    (input_size:   Nat)
+    (output_index: Nat)
+    (output_size:  Nat)
+    (code : ByteArray)
+    (disablePrecompiles: Bool)
+    (xl : Xlot)
+    (ex : Execution) : Prop :=
+    ExistsEq {devm with returnData := []} <|
+  λ evm1 =>
+    if (sevm.depth + 1 > 1024) then
+      (({evm1 with gasLeft := evm1.gasLeft + gas}).push 0 = ex)
+    else
+    ExistsEq (evm1.memory.data.sliceD input_index input_size 0) <|
+  λ calldata =>
+    ExistsEq
+      {
+        benv := {state := evm1.state, createdAccounts := evm1.createdAccounts, stat := sevm.benvStat}
+        tenv := {transientStorage := evm1.transientStorage, stat := sevm.tenvStat}
+        caller := caller
+        target := target
+        gas := gas
+        currentTarget := target
+        value := value
+        data := calldata
+        codeAddress := codeAddress
+        code := code
+        depth := sevm.depth + 1
+        shouldTransferValue := shouldTransferValue
+        isStatic := isStaticcall || sevm.isStatic
+        accessedAddresses := evm1.accessedAddresses
+        accessedStorageKeys := evm1.accessedStorageKeys
+        disablePrecompiles := disablePrecompiles
+      } <|
+    λ (childMsg : Msg) =>
+    ∃ ex',
+      And (ProcessMessage childMsg xl ex') <|
+      (liftToExecution evm1 ex').Split ex <|
+    λ child =>
+      let actualOutput := child.output.take output_size
+      if child.error.isSome then
+        ((incorporateChildOnError evm1 child child.output).push 0).Split ex <|
+      λ evm2 => .ok (evm2.memWrite output_index actualOutput) = ex
+      else
+        ((incorporateChildOnSuccess evm1 child child.output).push 1).Split ex <|
+      λ evm2 => .ok (evm2.memWrite output_index actualOutput) = ex
+
+def Ninst.Run' (pc : Nat) (sevm : Sevm) (devm : Devm) :
+    Ninst → Xlot → Except (String × Devm) (Nat × Devm) → Prop
+  | .push xs _, _, ex =>
+    ( do let devm1 ← chargeGas (if xs = [] then gBase else gVerylow) devm
+         let devm2 ← devm1.push xs.toB256
+         .ok ⟨pc + xs.length + 1, devm2⟩ ) = ex
+  | .reg r, _, ex => (Rinst.run ⟨pc, sevm, devm⟩ r).withPc (pc + 1) = ex
+  | .exec .create, xl, ex =>
+      (devm.pop).Split ex <|
+    λ ⟨endowment, devm1⟩ =>
+      (devm1.popToNat).Split ex <|
+    λ ⟨memoryIndex, devm2⟩ =>
+      (devm2.popToNat).Split ex <|
+    λ ⟨memorySize, devm3⟩ =>
+      ExistsEq (devm3.extCost [⟨memoryIndex, memorySize⟩]) <|
+    λ extendCost =>
+      ExistsEq (gasInitCodeWordCost * (ceilDiv memorySize 32)) <|
+    λ initCodeCost =>
+      (chargeGas (gasCreate + extendCost + initCodeCost) devm3).Split ex <|
+    λ devm4 =>
+      ExistsEq (devm4.memExtends [⟨memoryIndex, memorySize⟩]) <|
+    λ devm5 =>
+      ExistsEq
+        ( compute_contract_address
+            sevm.currentTarget
+            (devm5.state.get sevm.currentTarget).nonce ) <|
+    λ newAddress =>
+    ∃ ex',
+      And
+        ( GenericCreate
+            sevm
+            devm5
+            endowment
+            newAddress
+            memoryIndex
+            memorySize
+            xl
+            ex' ) <|
+      ex'.Split ex <|
+    λ devm6 =>
+      .ok ⟨pc + 1, devm6⟩ = ex
+  | .exec .create2, xl, ex =>
+      (devm.pop).Split ex <|
+    λ ⟨endowment, devm1⟩ =>
+      (devm1.popToNat).Split ex <|
+    λ ⟨memoryIndex, devm2⟩ =>
+      (devm2.popToNat).Split ex <|
+    λ ⟨memorySize, devm3⟩ =>
+      (devm3.pop).Split ex <|
+    λ ⟨salt, devm4⟩ =>
+      ExistsEq (devm4.extCost [⟨memoryIndex, memorySize⟩]) <|
+    λ extendCost =>
+      ExistsEq (gasKeccak256Word * ceilDiv memorySize 32) <|
+    λ initCodeHashCost =>
+      ExistsEq (gasInitCodeWordCost * (ceilDiv memorySize 32)) <|
+    λ initCodeCost =>
+      (chargeGas (gasCreate + initCodeHashCost + extendCost + initCodeCost) devm4).Split ex <|
+    λ devm5 =>
+      ExistsEq (devm5.memExtends [⟨memoryIndex, memorySize⟩]) <|
+    λ devm6 =>
+      ExistsEq
+        ( create2NewAddress
+            sevm.currentTarget
+            salt
+            (devm6.memory.data.sliceD memoryIndex memorySize 0) ) <|
+    λ newAddress =>
+    ∃ ex',
+      And
+        ( GenericCreate
+            sevm
+            devm6
+            endowment
+            newAddress
+            memoryIndex
+            memorySize
+            xl
+            ex' ) <|
+      ex'.Split ex <|
+    λ devm7 =>
+      .ok ⟨pc + 1, devm7⟩ = ex
+  | .exec .call, xl, ex =>
+      (devm.pop).Split ex <|
+    λ ⟨gas, devm1⟩ =>
+      (devm1.popToAdr).Split ex <|
+    λ ⟨callee, devm2⟩ =>
+      (devm2.pop).Split ex <|
+    λ ⟨value, devm3⟩ =>
+      (devm3.popToNat).Split ex <|
+    λ ⟨inputIndex, devm4⟩ =>
+      (devm4.popToNat).Split ex <|
+    λ ⟨inputSize, devm5⟩ =>
+      (devm5.popToNat).Split ex <|
+    λ ⟨outputIndex, devm6⟩ =>
+      (devm6.popToNat).Split ex <|
+    λ ⟨outputSize, devm7⟩ =>
+      ExistsEq (devm7.extCost [⟨inputIndex, inputSize⟩, ⟨outputIndex, outputSize⟩]) <|
+    λ extendCost =>
+      ExistsEq (access_cost callee devm7.accessedAddresses) <|
+    λ preAccessCost =>
+      ExistsEq (addAccessedAddress devm7 callee) <|
+    λ devm8 =>
+      ExistsEq (accessDelegation devm8 callee) <|
+    λ ⟨disablePrecompiles, _, code, delegatedAccessGasCost, devm9⟩ =>
+      ExistsEq (preAccessCost + delegatedAccessGasCost) <|
+    λ accessCost =>
+      ExistsEq (if (¬ (devm9.getAcct callee).Empty) ∨ value = 0 then 0 else gNewAccount) <|
+    λ createCost =>
+      ExistsEq (if value = 0 then 0 else gasCallValue) <|
+    λ transferCost =>
+      ExistsEq (calculateMsgCallGas value.toNat gas.toNat devm9.gasLeft extendCost (accessCost + createCost + transferCost)) <|
+    λ ⟨msgCallCost, msgCallStipend⟩ =>
+      (chargeGas (msgCallCost + extendCost) devm9).Split ex <|
+    λ devm10 =>
+      (Except.assert (!sevm.isStatic ∨ value = 0) ⟨"WriteInStaticContext", devm10⟩).Split ex <|
+    λ _ =>
+      ExistsEq (devm10.memExtends [⟨inputIndex, inputSize⟩, ⟨outputIndex, outputSize⟩]) <|
+    λ devm11 =>
+      ExistsEq ((devm11.getAcct sevm.currentTarget).bal) <|
+    λ senderBal =>
+      if senderBal < value then
+          (devm11.push 0).Split ex <|
+        λ devm12 =>
+          .ok ⟨pc + 1, {devm12 with returnData := [], gasLeft := devm12.gasLeft + msgCallStipend}⟩ = ex
+      else
+    ∃ ex',
+      And
+        ( GenericCall
+            sevm
+            devm11
+            msgCallStipend
+            value
+            sevm.currentTarget
+            callee
+            callee
+            true
+            false
+            inputIndex
+            inputSize
+            outputIndex
+            outputSize
+            code
+            disablePrecompiles
+            xl
+            ex' ) <|
+      ex'.Split ex <|
+    λ devm12 =>
+      .ok ⟨pc + 1, devm12⟩ = ex
+  | .exec .callcode, xl, ex =>
+      (devm.pop).Split ex <|
+    λ ⟨gas, devm1⟩ =>
+      (devm1.popToAdr).Split ex <|
+    λ ⟨codeAddress, devm2⟩ =>
+      (devm2.pop).Split ex <|
+    λ ⟨value, devm3⟩ =>
+      (devm3.popToNat).Split ex <|
+    λ ⟨inputIndex, devm4⟩ =>
+      (devm4.popToNat).Split ex <|
+    λ ⟨inputSize, devm5⟩ =>
+      (devm5.popToNat).Split ex <|
+    λ ⟨outputIndex, devm6⟩ =>
+      (devm6.popToNat).Split ex <|
+    λ ⟨outputSize, devm7⟩ =>
+      ExistsEq (devm7.extCost [⟨inputIndex, inputSize⟩, ⟨outputIndex, outputSize⟩]) <|
+    λ extendCost =>
+      ExistsEq (access_cost codeAddress devm7.accessedAddresses) <|
+    λ preAccessCost =>
+      ExistsEq (addAccessedAddress devm7 codeAddress) <|
+    λ devm8 =>
+      ExistsEq (accessDelegation devm8 codeAddress) <|
+    λ ⟨disablePrecompiles, newCodeAddress, code, delegatedAccessGasCost, devm9⟩ =>
+      ExistsEq (preAccessCost + delegatedAccessGasCost) <|
+    λ accessCost =>
+      ExistsEq (if value = 0 then 0 else gasCallValue) <|
+    λ transferCost =>
+      ExistsEq (calculateMsgCallGas value.toNat gas.toNat devm9.gasLeft extendCost (accessCost + transferCost)) <|
+    λ ⟨msgCallCost, msgCallStipend⟩ =>
+      (chargeGas (msgCallCost + extendCost) devm9).Split ex <|
+    λ devm10 =>
+      ExistsEq (devm10.memExtends [⟨inputIndex, inputSize⟩, ⟨outputIndex, outputSize⟩]) <|
+    λ devm11 =>
+      ExistsEq (devm11.getAcct sevm.currentTarget).bal <|
+    λ senderBal =>
+      if senderBal < value then
+          (devm11.push 0).Split ex <|
+        λ devm12 =>
+          .ok ⟨pc + 1, {devm12 with returnData := [], gasLeft := devm12.gasLeft + msgCallStipend}⟩ = ex
+      else
+    ∃ ex',
+      And
+        ( GenericCall
+            sevm
+            devm11
+            msgCallStipend
+            value
+            sevm.currentTarget
+            sevm.currentTarget
+            newCodeAddress
+            true
+            false
+            inputIndex
+            inputSize
+            outputIndex
+            outputSize
+            code
+            disablePrecompiles
+            xl
+            ex' ) <|
+      ex'.Split ex <|
+    λ devm12 =>
+      .ok ⟨pc + 1, devm12⟩ = ex
+  | .exec .delcall, xl, ex =>
+      (devm.pop).Split ex <|
+    λ ⟨gas, devm1⟩ =>
+      (devm1.popToAdr).Split ex <|
+    λ ⟨codeAddress, devm2⟩ =>
+      (devm2.popToNat).Split ex <|
+    λ ⟨inputIndex, devm3⟩ =>
+      (devm3.popToNat).Split ex <|
+    λ ⟨inputSize, devm4⟩ =>
+      (devm4.popToNat).Split ex <|
+    λ ⟨outputIndex, devm5⟩ =>
+      (devm5.popToNat).Split ex <|
+    λ ⟨outputSize, devm6⟩ =>
+      ExistsEq (devm6.extCost [⟨inputIndex, inputSize⟩, ⟨outputIndex, outputSize⟩]) <|
+    λ extendCost =>
+      ExistsEq (access_cost codeAddress devm6.accessedAddresses) <|
+    λ preAccessCost =>
+      ExistsEq (addAccessedAddress devm6 codeAddress) <|
+    λ devm7 =>
+      ExistsEq (accessDelegation devm7 codeAddress) <|
+    λ ⟨disablePrecompiles, newCodeAddress, code, delegatedAccessGasCost, devm8⟩ =>
+      ExistsEq (preAccessCost + delegatedAccessGasCost) <|
+    λ accessCost =>
+      ExistsEq (calculateMsgCallGas 0 gas.toNat devm8.gasLeft extendCost accessCost) <|
+    λ ⟨msgCallCost, msgCallStipend⟩ =>
+      (chargeGas (msgCallCost + extendCost) devm8).Split ex <|
+    λ devm9 =>
+      ExistsEq (devm9.memExtends [⟨inputIndex, inputSize⟩, ⟨outputIndex, outputSize⟩]) <|
+    λ devm10 =>
+    ∃ ex',
+      And
+        ( GenericCall
+            sevm
+            devm10
+            msgCallStipend
+            sevm.value
+            sevm.caller
+            sevm.currentTarget
+            newCodeAddress
+            false
+            false
+            inputIndex
+            inputSize
+            outputIndex
+            outputSize
+            code
+            disablePrecompiles
+            xl
+            ex' ) <|
+      ex'.Split ex <|
+    λ devm11 =>
+      .ok ⟨pc + 1, devm11⟩ = ex
+  | .exec .statcall, xl, ex =>
+      (devm.pop).Split ex <|
+    λ ⟨gas, devm1⟩ =>
+      (devm1.popToAdr).Split ex <|
+    λ ⟨target, devm2⟩ =>
+      (devm2.popToNat).Split ex <|
+    λ ⟨inputIndex, devm3⟩ =>
+      (devm3.popToNat).Split ex <|
+    λ ⟨inputSize, devm4⟩ =>
+      (devm4.popToNat).Split ex <|
+    λ ⟨outputIndex, devm5⟩ =>
+      (devm5.popToNat).Split ex <|
+    λ ⟨outputSize, devm6⟩ =>
+      ExistsEq (devm6.extCost [⟨inputIndex, inputSize⟩, ⟨outputIndex, outputSize⟩]) <|
+    λ extendCost =>
+      ExistsEq (access_cost target devm6.accessedAddresses) <|
+    λ preAccessCost =>
+      ExistsEq (addAccessedAddress devm6 target) <|
+    λ devm7 =>
+      ExistsEq (accessDelegation devm7 target) <|
+    λ ⟨disablePrecompiles, _, code, delegatedAccessGasCost, devm8⟩ =>
+      ExistsEq (preAccessCost + delegatedAccessGasCost) <|
+    λ accessCost =>
+      ExistsEq (calculateMsgCallGas 0 gas.toNat devm8.gasLeft extendCost accessCost) <|
+    λ ⟨msgCallCost, msgCallStipend⟩ =>
+      (chargeGas (msgCallCost + extendCost) devm8).Split ex <|
+    λ devm9 =>
+      ExistsEq (devm9.memExtends [⟨inputIndex, inputSize⟩, ⟨outputIndex, outputSize⟩]) <|
+    λ devm10 =>
+    ∃ ex',
+      And
+        ( GenericCall
+            sevm
+            devm10
+            msgCallStipend
+            0
+            sevm.currentTarget
+            target
+            target
+            true
+            true
+            inputIndex
+            inputSize
+            outputIndex
+            outputSize
+            code
+            disablePrecompiles
+            xl
+            ex' ) <|
+      ex'.Split ex <|
+    λ devm11 =>
+      .ok ⟨pc + 1, devm11⟩ = ex
+
+def Except.IsError {ξ υ : Type} (e : Except ξ υ) : Prop :=
+  match e with
+  | .error _ => True
+  | .ok _ => False
+
+/- Exec evm ex is provable iff
+    ∃ lim : Nat, ∀ vb : bool, exec vb lim evm = ex
+   holds, and ex is not a recursion limit error case.  -/
+inductive Exec : Nat → Sevm → Devm → Execution → Type
+  | invOp {pc} {sevm} {devm} :
+    sevm.code.getInst pc = none →
+    Exec pc sevm devm (.error ⟨"InvalidOpcode", devm⟩)
+  | nextNoneErr {pc} {sevm} {devm} {n : Ninst} {err} {devm'} :
+    n.At sevm.code pc →
+    Ninst.Run' pc sevm devm n .none (.error ⟨err, devm'⟩) →
+    Exec pc sevm devm (.error ⟨err, devm'⟩)
+  | nextSomeErr {pc} {sevm} {devm}
+    {n : Ninst} {evm} {exn} {err} {devm'} :
+    n.At sevm.code pc →
+    Ninst.Run' pc sevm devm n (.some (evm, exn)) (.error ⟨err, devm'⟩) →
+    Exec evm.pc evm.sta evm.dyna exn →
+    Exec pc sevm devm (.error ⟨err, devm'⟩)
+  | nextNoneRec {pc} {sevm : Sevm} {devm} {n : Ninst}
+    {pc'} {devm'} {exn : Execution} :
+    n.At sevm.code pc→
+    Ninst.Run' pc sevm devm n .none (.ok ⟨pc', devm'⟩) →
+    Exec pc' sevm devm' exn →
+    Exec pc sevm devm exn
+  | nextSomeRec {pc} {sevm} {devm} {n : Ninst} {evm' : Evm}
+    {exn' : Execution} {pc'} {devm'} {exn : Execution} :
+    n.At sevm.code pc→
+    Ninst.Run' pc sevm devm n (.some (evm', exn')) (.ok ⟨pc', devm'⟩) →
+    Exec evm'.pc evm'.sta evm'.dyna exn' →
+    Exec pc' sevm devm' exn →
+    Exec pc sevm devm exn
+  | jumpErr {pc} {sevm} {devm} {j : Jinst} {err} {devm'} :
+    j.At sevm.code pc →
+    Jinst.Run ⟨pc, sevm, devm⟩ j (.error ⟨err, devm'⟩) →
+    Exec pc sevm devm (.error ⟨err, devm'⟩)
+  | jumpRec {pc} {sevm} {devm} {j : Jinst} {pc'} {devm'} {exn} :
+    j.At sevm.code pc →
+    Jinst.Run ⟨pc, sevm, devm⟩ j (.ok ⟨pc', devm'⟩) →
+    Exec pc' sevm devm' exn →
+    Exec pc sevm devm exn
+  | last {pc} {sevm} {devm} {l : Linst} {exn : Execution} :
+    l.At sevm.code pc →
+    Linst.Run sevm devm l exn →
+    Exec pc sevm devm exn
+
+def Xlot.Filled : Xlot → Prop
+  | .none => True
+  | .some ⟨⟨pc, sevm, devm⟩, exn⟩ => Nonempty (Exec pc sevm devm exn)
+
+def Ninst.Run (sevm : Sevm) (devm : Devm) (n : Ninst)
+    (devm' : Devm) : Prop :=
+  ∃ xl : Xlot, xl.Filled ∧
+    ∃ pc pc', Ninst.Run' pc sevm devm n xl (.ok ⟨pc', devm'⟩)
+
+inductive Func.Run : List Func → Sevm → Devm → Func → Devm → Prop
+  | zero :
+    ∀ {fs sevm devm devm' f g devm''},
+      Devm.PopBurn [0] devm devm' →
+      Func.Run fs sevm devm' f devm'' →
+      Func.Run fs sevm devm (branch f g) devm''
+  | succ :
+    ∀ {fs sevm devm w devm' f g devm''},
+      w ≠ 0 →
+      Devm.PopBurn [w] devm devm' →
+      Func.Run fs sevm devm' g devm'' →
+      Func.Run fs sevm devm (branch f g) devm''
+  | last :
+    ∀ {fs sevm devm i devm' },
+      Linst.Run sevm devm i (.ok devm') →
+      Func.Run fs sevm devm (last i) devm'
+  | next :
+    ∀ {fs sevm devm i devm' f devm''},
+      Ninst.Run sevm devm i devm' →
+      Func.Run fs sevm devm' f devm'' →
+      Func.Run fs sevm devm (next i f) devm''
+  | call :
+    ∀ {fs sevm devm devm' k f devm''},
+      fs[k]? = some f →
+      Devm.Burn devm devm' →
+      Func.Run fs sevm devm' f devm'' →
+      Func.Run fs sevm devm (call k) devm'
+
+def Prog.Run (sevm : Sevm) (devm : Devm) (p : Prog) (devm' : Devm) : Prop :=
+  Func.Run (p.main :: p.aux) sevm devm p.main devm'
+
+-------------------------------------------------------------------------------
+
+def Except.toError? {ξ υ} : Except (String × ξ) υ → Option String
+  | .ok _ => none
+  | .error ⟨err, _⟩ => some err
+
+def Except.Lim {ξ υ} (ex : Except (String × ξ) υ) : Prop :=
+  ex.toError? = some "RecursionLimit"
+
+def Except.Fit {ξ υ} (ex : Except (String × ξ) υ) : Prop := ¬ ex.Lim
+
+def Xlot.Good' : Xlot → Prop
+  | .none => True
+  | .some (evm, ex) =>
+    ex.Fit ∧ ∃ lim, exec false evm lim = ex
+
+lemma of_lim_bind {ξ υ ζ} {x : Except (String × ξ) υ}
+    {f : υ → Except (String × ξ) ζ} (h : (x >>= f).Lim) :
+    x.Lim ∨ (∃ y, x = .ok y ∧ (f y).Lim) := by
+  rcases x with ⟨err, s⟩ | y
+  · left; simp [bind, Except.bind] at h; exact h
+  · right; use y; constructor; rfl
+    simp [bind, Except.bind] at h; exact h
+
+lemma fit_push {evm : Devm} {x : B256} : ¬ (evm.push x).Lim := by
+  unfold Except.Lim Devm.push Except.assert
+  split
+  · simp [Except.toError?, bind, Except.bind]
+  · simp [Except.toError?, bind, Except.bind]
+
+lemma fit_pop {evm : Devm} : ¬ evm.pop.Lim := by
+  simp only [Except.Lim, Devm.pop, Except.toError?]
+  cases evm.stack <;> simp
+
+lemma fit_popToNat {evm : Devm} : ¬ evm.popToNat.Lim := by
+  simp only [Except.Lim, Devm.popToNat, Except.toError?, Devm.pop]
+  cases evm.stack <;> simp
+
+lemma fit_pop_to_adr {evm : Devm} : ¬ evm.popToAdr.Lim := by
+  simp only [Except.Lim, Devm.popToAdr, Except.toError?, Devm.pop]
+  cases evm.stack <;> simp
+
+lemma fit_chargeGas {cost : Nat} {evm : Devm} :
+    ¬ (chargeGas cost evm).Lim := by
+  simp only [Except.Lim, Except.toError?, chargeGas]
+  cases safeSub evm.gasLeft cost <;> simp
+
+lemma fit_assert {p ξ} [Decidable p]
+    {s : String} {x : ξ} (ne : s ≠ "RecursionLimit") :
+    ¬ (Except.assert p ⟨s, x⟩).Lim := by
+  by_cases h : p <;>
+    simp [h, Except.assert, Except.toError?, Except.Lim, ne]
+
+lemma fit_assertDynamic {sevm : Sevm} {devm : Devm} :
+    ¬ (assertDynamic sevm devm).Lim := fit_assert (by decide)
+
+lemma fit_to_except {ξ υ} {x : ξ} {o : Option υ}
+    {s : String} (ne : s ≠ "RecursionLimit") :
+    ¬ (@Option.toExcept (String × ξ) υ ⟨s, x⟩ o).Lim := by
+  simp only [Except.Lim, Except.toError?, Option.toExcept]
+  cases o <;> simp [ne]
+
+lemma fit_ok {ξ υ} {y : υ} :
+    ¬ (.ok y : Except (String × ξ) υ).Lim := by intro h; cases h
+
+lemma fit_pushItem {x : B256} {c : Nat} {evm : Devm} :
+    ¬ (pushItem x c evm).Lim := by
+  simp only [pushItem]; intro run
+  rcases of_lim_bind run with run' | ⟨_, _, run'⟩
+  · cases fit_chargeGas run'
+  · cases fit_push run'
+
+lemma fit_applyUnary {f : B256 → B256} {cost : Nat} {devm : Devm} :
+    (applyUnary f cost devm).Fit := by
+  simp only [applyUnary]; intro run
+  rcases of_lim_bind run with run' | ⟨_, _, run'⟩
+  · cases fit_pop run'
+  · cases fit_pushItem run'
+
+syntax "fit_bind_step " ident term : tactic
+macro_rules
+  | `(tactic| fit_bind_step $ltd $lem) => `(tactic|
+      rcases of_lim_bind $ltd with ltd' | ⟨_, temp, ltd'⟩ <;>
+      [
+        (clear $ltd; apply $lem ltd' <;> clear ltd');
+        (clear $ltd temp; rename' ltd' => $ltd)
+      ]
+    )
+
+syntax "fit_bind_step' " ident term : tactic
+macro_rules
+  | `(tactic| fit_bind_step' $ltd $lem) => `(tactic|
+      rcases of_lim_bind $ltd with ltd' | ⟨_, temp, ltd'⟩;
+      swap; {apply $lem ltd'};
+      clear $ltd; rename' ltd' => $ltd
+    )
+
+lemma fit_applyBinary {f : B256 → B256 → B256} {cost : Nat} {evm : Devm} :
+    ¬ (applyBinary f cost evm).Lim := by
+  simp only [applyBinary]; intro ltd
+  fit_bind_step ltd fit_pop
+  fit_bind_step ltd fit_pop
+  cases fit_pushItem ltd
+
+lemma fit_applyTernary {f : B256 → B256 → B256 → B256} {cost : Nat} {evm : Devm} :
+    ¬ (applyTernary f cost evm).Lim := by
+  simp only [applyTernary]; intro ltd
+  fit_bind_step ltd fit_pop
+  fit_bind_step ltd fit_pop
+  fit_bind_step ltd fit_pop
+  cases fit_pushItem ltd
+
+lemma of_lim_map_rev {ξ υ ζ} {x : Except (String × ξ) υ}
+    {f : υ → ζ} (ltd : (x <&> f).Lim) : x.Lim := by
+  cases x <;> simp [Except.toError?, Except.Lim] at *; exact ltd
+
+lemma fit_pop_n {evm : Devm} {n : Nat} : ¬ (evm.popN n).Lim := by
+  induction n generalizing evm
+  case zero =>
+    simp [Devm.popN, Except.Lim, Except.toError?]
+  case succ n ih =>
+    simp only [Devm.popN]; intro ltd
+    fit_bind_step ltd fit_pop
+    fit_bind_step ltd ih; cases ltd
+
+lemma Rinst.fit_run {evm : Evm} {r : Rinst} :
+    (Rinst.run evm r).Fit := by
+  intro ltd; cases r <;> simp only [Rinst.run, Rinst.runCore] at ltd
+  case add => exact fit_applyBinary ltd
+  case mul => exact fit_applyBinary ltd
+  case sub => exact fit_applyBinary ltd
+  case div => exact fit_applyBinary ltd
+  case sdiv => exact fit_applyBinary ltd
+  case mod => exact fit_applyBinary ltd
+  case smod => exact fit_applyBinary ltd
+  case addmod => exact fit_applyTernary ltd
+  case mulmod => exact fit_applyTernary ltd
+  case exp =>
+    fit_bind_step ltd fit_pop
+    fit_bind_step ltd fit_pop
+    fit_bind_step ltd fit_chargeGas
+    exact fit_push ltd
+
+  case signextend => exact fit_applyBinary ltd
+  case lt => exact fit_applyBinary ltd
+  case gt => exact fit_applyBinary ltd
+  case slt => exact fit_applyBinary ltd
+  case sgt => exact fit_applyBinary ltd
+  case eq => exact fit_applyBinary ltd
+  case iszero =>
+    exact fit_applyUnary ltd
+  case and => exact fit_applyBinary ltd
+  case or => exact fit_applyBinary ltd
+  case xor => exact fit_applyBinary ltd
+  case not => exact fit_applyUnary ltd
+  case byte => exact fit_applyBinary ltd
+  case shr => exact fit_applyBinary ltd
+  case shl => exact fit_applyBinary ltd
+  case sar => exact fit_applyBinary ltd
+  case kec =>
+    fit_bind_step ltd fit_popToNat
+    fit_bind_step ltd fit_popToNat
+    fit_bind_step ltd fit_chargeGas
+    exact fit_push ltd
+  case address => exact fit_pushItem ltd
+  case balance =>
+    fit_bind_step ltd fit_pop
+    split at ltd <;>
+    { fit_bind_step ltd fit_chargeGas;
+      exact fit_push ltd }
+  case origin => exact fit_pushItem ltd
+  case caller => exact fit_pushItem ltd
+  case callvalue => exact fit_pushItem ltd
+  case calldataload =>
+    fit_bind_step ltd fit_pop
+    fit_bind_step ltd fit_chargeGas
+    exact fit_push ltd
+  case calldatasize => exact fit_pushItem ltd
+  case calldatacopy =>
+    fit_bind_step ltd fit_popToNat
+    fit_bind_step ltd fit_popToNat
+    fit_bind_step ltd fit_popToNat
+    fit_bind_step ltd fit_chargeGas
+    simp [Except.toError?, Except.Lim] at ltd
+  case codesize => exact fit_pushItem ltd
+  case codecopy =>
+    fit_bind_step ltd fit_popToNat
+    fit_bind_step ltd fit_popToNat
+    fit_bind_step ltd fit_popToNat
+    fit_bind_step ltd fit_chargeGas
+    simp [Except.toError?, Except.Lim] at ltd
+  case gasprice => exact fit_pushItem ltd
+  case extcodesize =>
+    fit_bind_step ltd fit_pop_to_adr
+    split at ltd <;> fit_bind_step ltd fit_chargeGas
+    · exact fit_push ltd
+    · exact fit_push ltd
+  case extcodecopy =>
+    fit_bind_step ltd fit_pop_to_adr
+    fit_bind_step ltd fit_popToNat
+    fit_bind_step ltd fit_popToNat
+    fit_bind_step ltd fit_popToNat
+    split at ltd <;> fit_bind_step ltd fit_chargeGas
+    · simp [Except.toError?, Except.Lim] at ltd
+    · simp [Except.toError?, Except.Lim] at ltd
+  case retdatasize => exact fit_pushItem ltd
+  case retdatacopy =>
+    fit_bind_step ltd fit_popToNat
+    fit_bind_step ltd fit_popToNat
+    fit_bind_step ltd fit_popToNat
+    fit_bind_step ltd fit_chargeGas
+    split at ltd <;> rename_i h_retdat
+    · simp only [bind, Except.bind, Except.Lim, Except.toError?] at ltd;
+      injection ltd; contradiction
+    · simp [Except.toError?, Except.Lim] at ltd
+  case extcodehash =>
+    fit_bind_step ltd fit_pop_to_adr
+    split at ltd <;> fit_bind_step ltd fit_chargeGas
+    · exact fit_push ltd
+    · exact fit_push ltd
+  case blockhash =>
+    fit_bind_step ltd fit_pop
+    fit_bind_step ltd fit_chargeGas
+    exact fit_push ltd
+  case coinbase => exact fit_pushItem ltd
+  case timestamp => exact fit_pushItem ltd
+  case number => exact fit_pushItem ltd
+  case prevrandao => exact fit_pushItem ltd
+  case gaslimit => exact fit_pushItem ltd
+  case chainid => exact fit_pushItem ltd
+  case selfbalance => exact fit_pushItem ltd
+  case basefee => exact fit_pushItem ltd
+  case blobhash =>
+    fit_bind_step ltd fit_pop
+    fit_bind_step ltd fit_chargeGas
+    exact fit_push ltd
+  case blobbasefee => exact fit_pushItem ltd
+  case pop =>
+    fit_bind_step' ltd fit_chargeGas
+    exact fit_pop <| of_lim_map_rev ltd
+  case mload =>
+    fit_bind_step ltd fit_popToNat
+    fit_bind_step ltd fit_chargeGas
+    exact fit_push ltd
+  case mstore =>
+    fit_bind_step ltd fit_popToNat
+    fit_bind_step ltd fit_pop
+    fit_bind_step ltd fit_chargeGas
+    simp [Except.toError?, Except.Lim] at ltd
+  case mstore8 =>
+    fit_bind_step ltd fit_popToNat
+    fit_bind_step ltd fit_pop
+    fit_bind_step ltd fit_chargeGas
+    simp [Except.toError?, Except.Lim] at ltd
+  case sload =>
+    fit_bind_step ltd fit_pop
+    split at ltd <;> fit_bind_step ltd fit_chargeGas
+    · exact fit_push ltd
+    · exact fit_push ltd
+  case sstore =>
+    fit_bind_step ltd fit_pop
+    fit_bind_step ltd fit_pop
+    have ne : "OutOfGasError" ≠ "RecursionLimit" := by decide
+    fit_bind_step ltd (fit_assert ne)
+    fit_bind_step ltd fit_chargeGas
+    fit_bind_step ltd fit_assertDynamic
+    cases ltd
+  case tload =>
+    fit_bind_step ltd fit_pop
+    exact fit_pushItem ltd
+  case tstore =>
+    fit_bind_step ltd fit_pop
+    fit_bind_step ltd fit_pop
+    fit_bind_step ltd fit_chargeGas
+    fit_bind_step ltd fit_assertDynamic
+    cases ltd
+  case mcopy =>
+    fit_bind_step ltd fit_popToNat
+    fit_bind_step ltd fit_popToNat
+    fit_bind_step ltd fit_popToNat
+    fit_bind_step ltd fit_chargeGas
+    cases ltd
+  case pc => exact fit_pushItem ltd
+  case msize => exact fit_pushItem ltd
+  case gas =>
+    fit_bind_step ltd fit_chargeGas
+    exact fit_push ltd
+  case dup =>
+    fit_bind_step ltd fit_chargeGas
+    split at ltd
+    · simp [Except.toError?, Except.Lim] at ltd
+    · exact fit_push ltd
+  case swap =>
+    fit_bind_step ltd fit_chargeGas
+    split at ltd
+    · simp [Except.toError?, Except.Lim] at ltd
+    · cases ltd
+  case log =>
+    fit_bind_step ltd fit_popToNat
+    fit_bind_step ltd fit_popToNat
+    fit_bind_step ltd fit_pop_n
+    fit_bind_step ltd fit_chargeGas
+    fit_bind_step ltd fit_assertDynamic
+    cases ltd
+
+lemma Except.of_error_bind_eq {ξ υ ζ : Type}
+    {x : ξ} {f : υ → Except ξ ζ} (e : Except ξ ζ)
+    (eq : (Except.error x) >>= f = e) : Except.error x = e := by
+  simp [bind, Except.bind] at eq; exact eq
+
+lemma error_bind {ξ υ ζ : Type}
+    {x : ξ} {f : υ → Except ξ ζ} :
+    (Except.error x) >>= f = Except.error x := rfl
+
+def ok_bind {ξ : Type u} {υ ζ : Type v} {y : υ} {g : υ → Except ξ ζ} :
+    (.ok y) >>= g = g y := rfl
+
+lemma fit_withPc {pc : ℕ} {exn : Execution} (fit : exn.Fit) :
+    (exn.withPc pc).Fit := by
+  simp only [Execution.withPc]
+  rcases exn with ⟨err, devm⟩ | _
+  · rw [error_bind]; exact fit
+  · rw [ok_bind]; exact fit
+
+lemma forall_gt_of_forall_gt_succ_pred {p : Nat → Prop} (n : Nat) :
+    (∀ m > n, p (m.pred + 1)) → (∀ m > n, p m) := by
+  intro fa m gt; rcases m with _ | m
+  · cases Nat.not_lt_zero _ gt
+  · apply fa (m + 1) gt
+
+lemma fit_of_split_of_fit {ξ υ ζ} {x : Except (String × ξ) υ}
+    {p : υ → Prop} {ex : Except (String × ξ) ζ}
+    (split : Except.Split x ex p) (fit : x.Fit) :
+    (∀ y, x = .ok y → p y → ex.Fit) → ex.Fit := by
+  intro prem
+  rcases split with ⟨⟨err, _⟩ , rw, rw'⟩ | ⟨y, eq, py⟩
+  · rw [rw']; intro ltd; injection ltd with rw''
+    rw [rw, rw''] at fit; cases fit rfl
+  · exact (prem _ eq py)
+
+syntax "fit_step_split " ident term : tactic
+macro_rules
+  | `(tactic| fit_step_split $run $lem) =>
+    `(tactic|
+      apply fit_of_split_of_fit $run $lem;
+      clear $run; intro _ temp $run; clear temp;
+    )
+
+syntax "fit_step_exists " ident : tactic
+macro_rules
+  | `(tactic| fit_step_exists $run) =>
+    `(tactic|
+      have temp := $run; clear $run;
+      rcases temp with ⟨_, temp, $run⟩; clear temp
+    )
+
+syntax "fit_step_exec " ident ident term:max term : tactic
+macro_rules
+  | `(tactic| fit_step_exec $run $good $lem $lem') =>
+    `(tactic|
+      have temp := $run; clear $run;
+      rcases temp with ⟨ex', runs, $run⟩;
+      have temp := $lem $good runs; clear $good runs;
+      rcases temp with ⟨fit, lim, run_eq⟩; clear lim run_eq;
+      fit_step_split $run ($lem' fit); clear fit
+    )
+
+lemma fit_benvAfterTransfer {msg : Msg} : msg.benvAfterTransfer.Fit := by
+  simp only [Msg.benvAfterTransfer]; intro ltd
+  split at ltd
+  · fit_bind_step ltd (fit_to_except (by decide)); exact fit_ok ltd
+  · exact fit_ok ltd
+
+lemma of_lim_handleError {ex : Execution} :
+    (executeCode.handleError ex).Lim → ex.Lim := by
+  rcases ex with ⟨err, err⟩ | _ <;>
+    simp only [executeCode.handleError] <;> intro h
+  · split at h; {cases h}; split at h; {cases h}; exact h
+  · exact h
+
+def Saturates {ξ υ} (n : Nat) (f : Nat → Except (String × ξ) υ) : Prop :=
+  (f n).Fit → ∀ m, n < m → (f n = f m)
+
+structure Saturation (lim : Nat) : Prop where
+  (executeCode : ∀ (msg : Msg), Saturates lim (executeCode false msg))
+  (processMessage : ∀ (msg : Msg), Saturates lim (processMessage false msg))
+  ( processCreateMessage :
+    ∀ (msg : Msg), Saturates lim (processCreateMessage false msg) )
+  ( genericCreate :
+    ∀ (sevm : Sevm) (devm : Devm)
+      (endowment : B256) (newAddress : Adr)
+      (memoryIndex : Nat) (memorySize : Nat),
+      Saturates lim
+        (genericCreate false sevm devm endowment newAddress memoryIndex memorySize) )
+  ( genericCall :
+    ∀ (sevm : Sevm) (devm : Devm)
+      (gas : Nat) (value : B256) (caller : Adr) (target : Adr)
+      (codeAddress : Adr) (shouldTransferValue : Bool) (isStaticcall : Bool)
+      (inputIndex :Nat) (inputSize : Nat) (outputIndex : Nat)
+      (outputSize : Nat) (code : ByteArray) (disablePrecompiles: Bool),
+      Saturates lim
+        ( genericCall false sevm devm gas value caller target codeAddress
+            shouldTransferValue isStaticcall inputIndex inputSize outputIndex
+            outputSize code disablePrecompiles ) )
+  (run : ∀ (evm : Evm) (n : Ninst), Saturates lim (Ninst.run false evm n))
+  (exec : ∀ (evm : Evm), Saturates lim (exec false evm))
+
+lemma lim_handleError {ex : Execution} :
+    ex.Lim → (executeCode.handleError ex).Lim := by
+  intro h; rcases ex with ⟨err, err⟩ | _ <;>
+    simp [Except.Lim, Except.toError?] at h
+  rw [h]; rfl
+
+lemma Except.bind_eq_bind {ξ υ ζ} {e : Except ξ υ} {f g : υ → Except ξ ζ}
+    (eq : ∀ x, e = Except.ok x → f x = g x) : e >>= f = e >>= g := by
+  cases e; rfl; apply eq _ rfl
+
+lemma of_fit_bind {ξ υ ζ} {x : Except (String × ξ) υ}
+    {f : υ → Except (String × ξ) ζ} (fit : (x >>= f).Fit) :
+    x.Fit ∧ (∀ y, x = .ok y → (f y).Fit) := by
+  constructor
+  · intro ltd
+    rcases x with ⟨_, _⟩ | _
+    · injection ltd; rename_i rw; rw [rw] at fit; cases fit rfl
+    · cases ltd
+  · intro y eq; rw [eq] at fit; exact fit
+
+syntax "eee_bind " ident  : tactic
+macro_rules
+  | `(tactic| eee_bind $fit) => `(tactic|
+      apply Except.bind_eq_bind;
+      intro _ eq_ok;
+      have temp := $fit; clear $fit;
+      have $fit :=
+        @Eq.subst _ (Except.Fit) _ _ ok_bind <|
+          @Eq.subst _ (λ e => Except.Fit (e >>= _)) _ _ eq_ok temp;
+      clear temp eq_ok
+    )
+
+lemma of_fit_liftToExecution {evm : Devm}
+    {f : Except (String × State × AdrSet × Tra) Devm} :
+    (liftToExecution evm f).Fit → f.Fit := by
+  rcases f with ⟨err, _⟩ | _ <;> intro fit ltd
+  · injection ltd; rename_i rw; rw [rw] at fit; cases fit rfl
+  · cases ltd
+
+lemma saturation (lim : Nat) : Saturation lim := by
+  induction lim
+  case zero =>
+    refine' ⟨_, _, _, _, _, _, _⟩
+    · intro _ fit; simp only [executeCode] at fit; cases fit rfl
+    · intro _ fit; simp only [processMessage] at fit; cases fit rfl
+    · intro _ fit; simp only [processCreateMessage] at fit; cases fit rfl
+    · intro _ _ _ _ _ _ fit; simp only [genericCreate] at fit; cases fit rfl
+    · intro _ _ _ _ _ _ _ _ _ _ _ _ _ _ _ fit;
+      simp only [genericCall] at fit; cases fit rfl
+    · intro _ n fit; cases n
+      · simp only [Ninst.run, implies_true]
+      · simp only [Ninst.run] at fit; cases fit rfl
+      · simp only [Ninst.run, implies_true]
+    · intro _ fit; simp only [exec] at fit; cases fit rfl
+  case succ lim ih =>
+    refine' ⟨_, _, _, _, _, _, _⟩
+    · intro _ fit lim' lt
+      rcases lim' with _ | lim'; {cases Nat.not_lt_zero _ lt}
+      simp only [executeCode] at *
+      split at fit
+      · rw [ih.exec _ (lim_handleError.mt fit) lim' (by omega)]
+      · split at fit
+        · rename_i pos; rw [if_pos pos, if_pos pos]
+        · rename_i neg; rw [if_neg neg, if_neg neg]
+          rw [ih.exec _ (lim_handleError.mt fit) lim' (by omega)]
+    · intro _ fit lim' lt
+      rcases lim' with _ | lim'; {cases Nat.not_lt_zero _ lt}
+      simp only [processMessage] at *
+      eee_bind fit; eee_bind fit
+      rw [ih.executeCode _ (of_fit_bind fit).1 lim' (by omega)]
+    · intro _ fit lim' lt
+      rcases lim' with _ | lim'; {cases Nat.not_lt_zero _ lt}
+      simp only [processCreateMessage] at *
+      rw [ih.processMessage _ (of_fit_bind fit).1 lim' (by omega)]
+    · intro _ _ _ _ _ _ fit lim' lt
+      rcases lim' with _ | lim'; {cases Nat.not_lt_zero _ lt}
+      simp only [genericCreate] at *
+      iterate 8 (eee_bind fit);
+      split; {rfl}
+      rename_i neg; rw [if_neg neg] at fit; clear neg
+      eee_bind fit; eee_bind fit; split; {rfl}
+      rename_i neg; rw [if_neg neg] at fit; clear neg
+      eee_bind fit; eee_bind fit
+      have fit' := of_fit_liftToExecution (of_fit_bind fit).1
+      rw [ih.processCreateMessage _ fit' lim' (by omega)]
+    · intro _ _ _ _ _ _ _ _ _ _ _ _ _ _ _ fit lim' lt
+      rcases lim' with _ | lim'; {cases Nat.not_lt_zero _ lt}
+      simp only [genericCall] at *
+      eee_bind fit; split at fit
+      · rename_i pos; rw [if_pos pos, if_pos pos]
+      · rename_i neg; rw [if_neg neg, if_neg neg]
+        iterate 3 (eee_bind fit)
+        have fit' := of_fit_liftToExecution (of_fit_bind fit).1
+        rw [ih.processMessage _ fit' lim' (by omega)]
+    · intro _ n fit lim' lt
+      rcases lim' with _ | lim'; {cases Nat.not_lt_zero _ lt}
+      rcases n  with _ | (_ | _ | _ | _ | _ | _) | _ <;>
+        simp only [Ninst.run] at *
+      · iterate 8 (eee_bind fit)
+        rw [ih.genericCreate _ _ _ _ _ _ (of_fit_bind fit).1 lim' (by omega)]
+      · iterate 19 (eee_bind fit)
+        split; {rfl}; rename_i neg
+        rw [if_neg neg] at fit; clear neg
+        rw [ ih.genericCall _ _ _ _ _ _ _ _ _ _ _ _ _ _ _
+             (of_fit_bind fit).1 lim' (by omega) ]
+      · iterate 17 (eee_bind fit)
+        split; {rfl}; rename_i neg
+        rw [if_neg neg] at fit; clear neg
+        rw [ ih.genericCall _ _ _ _ _ _ _ _ _ _ _ _ _ _ _
+             (of_fit_bind fit).1 lim' (by omega) ]
+      · iterate 14 (eee_bind fit)
+        rw [ ih.genericCall _ _ _ _ _ _ _ _ _ _ _ _ _ _ _
+             (of_fit_bind fit).1 lim' (by omega) ]
+      · iterate 10 (eee_bind fit)
+        rw [ih.genericCreate _ _ _ _ _ _ (of_fit_bind fit).1 lim' (by omega)]
+      · iterate 14 (eee_bind fit)
+        rw [ ih.genericCall _ _ _ _ _ _ _ _ _ _ _ _ _ _ _
+             (of_fit_bind fit).1 lim' (by omega) ]
+    · intro _ fit lim' lt
+      rcases lim' with _ | lim'; {cases Nat.not_lt_zero _ lt}
+      simp only [exec] at *; eee_bind fit; split
+      · simp only at fit
+        rw [← ih.run _ _ (of_fit_bind fit).1 lim' (by omega)]
+        eee_bind fit; apply ih.exec _ fit lim' (by omega)
+      · simp only at fit; eee_bind fit
+        apply ih.exec _ fit lim' (by omega)
+      · rfl
+
+lemma fit_execute_ecrecover (evm : Evm) :
+    (executeEcrecover evm).Fit := by
+  intro ltd;
+  fit_bind_step ltd fit_chargeGas
+  fit_bind_step ltd fit_ok
+  split at ltd
+  · simp only [] at ltd
+    split at ltd; {cases ltd}
+    split at ltd <;> cases ltd
+  · cases ltd
+
+lemma fit_for_in {ξ υ} {xs : List Nat} {y : υ}
+    {f : Nat → υ → Except (String × ξ) (ForInStep υ)}
+    (fit : ∀ n y, (f n y).Fit) : (ForIn.forIn xs y f).Fit := by
+  induction xs generalizing y with
+    | nil => rw [List.forIn_nil]; intro ltd; cases ltd
+    | cons x xs ih =>
+      rw [List.forIn_cons]; intro ltd
+      fit_bind_step ltd (fit _ _); split at ltd
+      · cases ltd
+      · apply ih ltd
+
+lemma fit_catch_with_oog {ξ : Type U} {evm : Devm} {cond : String → Bool}
+    {ex : Except String ξ} (fit : ex ≠ .error "RecursionLimit") :
+    (catchWithOOG evm cond ex).Fit := by
+  simp only [catchWithOOG]; split
+  · apply fit_ok
+  · split <;> intro ltd <;> injection ltd
+    · contradiction
+    . rename_i rw; rw [rw] at fit; cases fit rfl
+
+lemma fit_toExStrBNP {xs} :
+    B8L.toExStrBNP xs ≠ .error "RecursionLimit" := by
+  simp only [B8L.toExStrBNP]; intro ltd
+  split at ltd; {injection ltd; contradiction}
+  split at ltd; {injection ltd; contradiction}
+  split at ltd; {injection ltd; contradiction}
+  simp [Option.toExcept] at ltd;
+  split at ltd; {injection ltd; contradiction}
+  cases ltd
+
+lemma fit_toExStrBNP2 {xs} :
+    B8L.toExStrBNP2 xs ≠ .error "RecursionLimit" := by
+  simp only [B8L.toExStrBNP2]; intro ltd
+  split at ltd; {injection ltd; contradiction}
+  split at ltd; {injection ltd; contradiction}
+  simp [Option.toExcept] at ltd;
+  split at ltd; {injection ltd; contradiction}
+  cases ltd
+
+lemma fit_execute_precomp (evm : Evm) (adr : Adr) :
+    (executePrecomp evm adr).Fit := by
+  simp only [executePrecomp]; split
+  · apply fit_execute_ecrecover
+  · intro ltd; fit_bind_step ltd fit_chargeGas; cases ltd
+  · intro ltd; fit_bind_step ltd fit_chargeGas; cases ltd
+  · intro ltd; fit_bind_step ltd fit_chargeGas; cases ltd
+  · intro ltd; fit_bind_step ltd fit_chargeGas
+    split at ltd <;> cases ltd
+  · intro ltd;
+    fit_bind_step ltd fit_chargeGas
+    fit_bind_step ltd (fit_assert (by decide))
+    fit_bind_step ltd (fit_to_except (by decide))
+    fit_bind_step ltd (fit_to_except (by decide))
+    cases ltd
+  · intro ltd; fit_bind_step ltd fit_chargeGas
+    fit_bind_step ltd (fit_assert (by decide))
+    fit_bind_step ltd (fit_to_except (by decide))
+    cases ltd
+  · intro ltd; fit_bind_step ltd fit_chargeGas
+    fit_bind_step ltd (fit_assert (by decide))
+    fit_bind_step ltd (fit_for_in _)
+    · intro n y ltd
+      fit_bind_step ltd (fit_catch_with_oog fit_toExStrBNP)
+      fit_bind_step ltd (fit_catch_with_oog fit_toExStrBNP2)
+      fit_bind_step ltd (fit_assert (by decide))
+      fit_bind_step ltd (fit_assert (by decide))
+      fit_bind_step ltd (fit_to_except (by decide))
+      cases ltd
+    · cases ltd
+  · intro ltd;
+    fit_bind_step ltd (fit_assert (by decide))
+    fit_bind_step ltd fit_chargeGas
+    split at ltd
+    · fit_bind_step ltd fit_ok
+      fit_bind_step ltd (fit_to_except (by decide))
+      cases ltd
+    · fit_bind_step ltd fit_ok
+      fit_bind_step ltd (fit_to_except (by decide))
+      cases ltd
+    · injection ltd; contradiction
+  · intro ltd
+    fit_bind_step ltd (fit_assert (by decide))
+    injection ltd; contradiction
+  · intro ltd
+    fit_bind_step ltd (fit_assert (by decide))
+    injection ltd; contradiction
+  · intro ltd; simp only [executeBls12G1Msm] at ltd
+    split at ltd
+    · injection ltd; rename_i eq
+      cases congr_arg String.head eq
+    · simp only [pure_bind] at ltd
+      fit_bind_step ltd fit_chargeGas
+      injection ltd; contradiction
+  · intro ltd; simp only [executeBls12G2Add] at ltd
+    split at ltd
+    · injection ltd; contradiction
+    · simp only [pure_bind] at ltd
+      fit_bind_step ltd fit_chargeGas
+      injection ltd; contradiction
+  · intro ltd; simp only [executeBls12G2Msm] at ltd
+    split at ltd
+    · injection ltd; rename_i eq
+      cases congr_arg String.head eq
+    · simp only [pure_bind] at ltd
+      fit_bind_step ltd fit_chargeGas
+      injection ltd; contradiction
+  · intro ltd; simp only [executeBls12Pairing] at ltd
+    split at ltd
+    · injection ltd; rename_i eq
+      cases congr_arg String.head eq
+    · simp only [pure_bind] at ltd
+      fit_bind_step ltd fit_chargeGas
+      injection ltd; contradiction
+  · intro ltd; simp only [executeBls12MapFpToG1] at ltd
+    split at ltd
+    · injection ltd; contradiction
+    · simp only [pure_bind] at ltd
+      fit_bind_step ltd fit_chargeGas
+      injection ltd; contradiction
+  · intro ltd; simp only [executeBls12MapFp2ToG2] at ltd
+    fit_bind_step ltd (fit_assert (by decide))
+    fit_bind_step ltd fit_chargeGas
+    injection ltd; contradiction
+  · intro ltd; injection ltd; rename_i eq
+    cases congr_arg String.head eq
+
+lemma of_execute_code' {msg : Msg} {xl : Xlot}
+    {ex : Except (String × State × AdrSet × Tra) Devm}
+    (good : xl.Good') (ec : ExecuteCode msg xl ex) :
+    ex.Fit ∧ ∃ lim, ∀ lim' > lim, executeCode false msg lim' = ex := by
+  simp only [ExecuteCode] at ec; split at ec
+  · rename (msg.codeAddress = none) => eq_none
+    rcases ec with ⟨ex', xl_eq, eq_ex⟩
+    rw [xl_eq] at good
+    simp [Xlot.Good'] at good
+    rcases good with ⟨fit', lim, eq_ex'⟩
+    have fit : ex.Fit := by
+      rw [← eq_ex]
+      exact (of_lim_handleError).mt fit'
+    refine' ⟨fit, lim + 1, _⟩
+    intro lim' gt
+    rcases lim' with _ | lim'; {cases Nat.not_lt_zero _ gt}
+    simp only [executeCode]
+    rw [eq_none]; simp only
+    rw [← eq_ex'] at fit'
+    rw [← (saturation lim).exec _ fit' lim' (by omega), eq_ex', eq_ex]
+  · rename Adr => adr
+    rename (msg.codeAddress = some adr) => eq_some
+    split at ec
+    · rename_i pos; constructor
+      · rw [← ec.2]; intro ltd
+        cases fit_execute_precomp _ _ <| of_lim_handleError ltd
+      · refine' ⟨1, _⟩; intro lim' gt
+        rcases lim' with _ | lim'; {cases Nat.not_lt_zero _ gt}
+        simp only [executeCode, eq_some, if_pos pos]; exact ec.2
+    · rename_i neg; rcases ec with ⟨ex', xl_eq, eq_ex⟩
+      rw [xl_eq] at good; simp [Xlot.Good'] at good
+      rcases good with ⟨fit, lim, eq_ex'⟩
+      constructor
+      · rw [← eq_ex]; intro ltd;
+        cases fit <| of_lim_handleError ltd
+      · refine' ⟨lim + 1, _⟩; intro lim' gt
+        rcases lim' with _ | lim'; {cases Nat.not_lt_zero _ gt}
+        simp only [executeCode]
+        rw [eq_some]; simp only
+        rw [if_neg neg]; rw [← eq_ex'] at fit
+        rw [← (saturation lim).exec _ fit lim' (by omega), eq_ex', eq_ex]
+
+lemma exists_forall_gt_ok_bind_eq {ξ υ ζ}
+    {f : Nat → υ → Except (String × ξ) ζ} {y : υ} {ex : Except (String × ξ) ζ} :
+    (∃ lim, ∀ lim' > lim, (f lim' y) = ex) →
+    ∃ lim, ∀ lim' > lim, (.ok y >>= f lim') = ex := id
+
+lemma exists_forall_gt_of_split {ξ υ ζ} {x : Except (String × ξ) υ}
+    {ex : Except (String × ξ) ζ} {p : υ → Prop}
+    {f : Nat → υ → Except (String × ξ) ζ} (split : Except.Split x ex p) :
+    (∀ y, x = .ok y → p y → ∃ lim, ∀ lim' > lim, (f lim' y) = ex) →
+    ∃ lim, ∀ lim' > lim, (x >>= f lim') = ex := by
+  intro prem
+  rcases split with ⟨⟨err, _⟩ , rw, rw'⟩ | ⟨y, eq, py⟩
+  · refine' ⟨0, _⟩; intro _ _; rw [rw, rw']; rfl
+  · rcases (prem _ eq py) with ⟨lim, fa⟩
+    refine' ⟨lim, _⟩; intro lim' gt; rw [eq]; apply fa _ gt
+
+syntax "efg_step_split " ident : tactic
+macro_rules
+  | `(tactic| efg_step_split $run) =>
+    `(tactic|
+      apply exists_forall_gt_of_split $run; clear $run;
+      intro _ temp $run; clear temp
+    )
+
+lemma bind_eq_of_eq_ok_of_eq {ξ υ ζ} {x : Except ξ υ} {y} {z : Except ξ ζ}
+    {f : υ → Except ξ ζ} (eq_ok : x = .ok y) (eq : f y = z) : (x >>= f) = z := by
+  rw [eq_ok]; exact eq
+
+syntax "eq_split " ident : tactic
+macro_rules
+  | `(tactic| eq_split $eq) => `(tactic|
+      have temp := $eq; clear $eq;
+      rcases temp with ⟨⟨_, _, _⟩, rw', rw⟩ | ⟨_, eq', $eq⟩ <;> [
+        (rw [rw', rw]; rfl);
+        (apply bind_eq_of_eq_ok_of_eq eq'; clear eq')
+      ]
+    )
+
+lemma ite_eq_left_of_true {ξ : Sort u} {C : Prop} [h : Decidable C]
+    {x y z : ξ} (c : C) (eq : x = z) : (if C then x else y) = z := by simp [c, eq]
+
+lemma ite_eq_right_of_false {ξ : Sort u} {C : Prop} [h : Decidable C]
+    {x y z : ξ} (c : ¬ C) (eq : y = z) : (if C then x else y) = z := by simp [c, eq]
+
+lemma or_of_ite {c p q : Prop} [h : Decidable c] (h : if c then p else q) :
+    (c ∧ p) ∨ (¬ c ∧ q) := by
+  by_cases hc : c <;> simp [hc] at h
+  · left; exact ⟨hc, h⟩
+  · right; exact ⟨hc, h⟩
+
+syntax "eq_ite " ident : tactic
+macro_rules
+  | `(tactic| eq_ite $eq) => `(tactic|
+      rename' $eq => temp;
+      rcases or_of_ite temp with ⟨pos, $eq⟩ | ⟨neg, $eq⟩ <;> clear temp <;>
+      [
+        (apply ite_eq_left_of_true pos; clear pos) ;
+        (apply ite_eq_right_of_false neg; clear neg)
+      ]
+    )
+
+lemma of_process_message' {msg : Msg} {xl : Xlot}
+    {ex : Except (String × State × AdrSet × Tra) Devm} (good : xl.Good')
+    (run : ProcessMessage msg xl ex) :
+    ex.Fit ∧ ∃ lim, ∀ lim' > lim, processMessage false msg lim' = ex := by
+  simp only [ProcessMessage] at run; constructor
+  · fit_step_split run (fit_assert (by decide))
+    fit_step_split run fit_benvAfterTransfer
+    fit_step_exec run good of_execute_code' id
+    split at run <;> (rw [← run]; apply fit_ok)
+  · apply Exists.imp forall_gt_of_forall_gt_succ_pred
+    simp only [processMessage]
+    efg_step_split run; efg_step_split run;
+    have temp := run; clear run;
+    rcases temp with ⟨ex', runs, run⟩;
+    have temp := of_execute_code' good runs;
+    clear good runs;
+    rcases temp with ⟨fit, lim, run_eq⟩;
+    clear fit;
+    refine' ⟨lim + 1, _⟩;
+    intro lim' gt;
+    have gt' : lim'.pred > lim :=
+    ( by cases lim' <;>
+         [ (cases Nat.not_lt_zero _ gt);
+           (exact Nat.lt_of_succ_lt_succ gt) ] );
+    rw [run_eq lim'.pred gt'];
+    clear gt gt' run_eq;
+    eq_split run;
+    eq_ite run <;> exact run
+
+lemma processCreateMessage.fit_chargeCodeGas {evm : Devm} :
+    (processCreateMessage.chargeCodeGas evm).Fit := by
+  simp only [processCreateMessage.chargeCodeGas]; intro ltd
+  split at ltd
+  · injection ltd; contradiction
+  · fit_bind_step ltd fit_chargeGas
+    split at ltd
+    · injection ltd; contradiction
+    · cases ltd
+
+syntax "efg_step_exec " ident ident term:max : tactic
+macro_rules
+  | `(tactic| efg_step_exec $run $good $lem) =>
+    `(tactic|
+      have temp := $run; clear $run;
+      rcases temp with ⟨ex', runs, $run⟩;
+      have temp := $lem $good runs;
+      clear $good runs;
+      rcases temp with ⟨fit, lim, run_eq⟩;
+      clear fit;
+      refine' ⟨lim + 1, _⟩;
+      intro lim' gt;
+      have gt' : lim'.pred > lim :=
+      ( by cases lim' <;>
+           [ (cases Nat.not_lt_zero _ gt);
+             (exact Nat.lt_of_succ_lt_succ gt) ] );
+      rw [run_eq lim'.pred gt'];
+      clear gt gt' run_eq;
+    )
+
+lemma of_process_create_message' {msg : Msg} {xl : Xlot}
+    {ex : Except (String × State × AdrSet × Tra) Devm} (good : xl.Good')
+    (run : ProcessCreateMessage msg xl ex) :
+    ex.Fit ∧
+      ∃ lim, ∀ lim' > lim, processCreateMessage false msg lim' = ex := by
+  simp only [ProcessCreateMessage] at run; constructor
+  · fit_step_exec run good of_process_message' id
+    rename Devm => evm; split at run
+    · split at run; {rw [← run]; apply fit_ok}
+      rename_i eq; split at run
+      · rw [← run]; apply fit_ok
+      · rw [← run]; intro ltd; injection ltd with rw
+        have fit := @processCreateMessage.fit_chargeCodeGas evm
+        rw [eq, rw] at fit; cases fit rfl
+    · rw [← run]; apply fit_ok
+  · apply Exists.imp forall_gt_of_forall_gt_succ_pred
+    simp only [processCreateMessage]
+    efg_step_exec run good of_process_message'
+    eq_split run; eq_ite run
+    · split at run <;> rename_i rw <;> rw [rw]
+      · exact run
+      · eq_ite run <;> exact run
+    · exact run
+
+syntax "efg_step_exists " ident : tactic
+macro_rules
+  | `(tactic| efg_step_exists $run) =>
+    `(tactic|
+      have temp := $run; clear $run;
+      rcases temp with ⟨_, rw, $run⟩;
+      rw [← rw]; clear rw;
+      apply exists_forall_gt_ok_bind_eq
+    )
+
+lemma exists_forall_gt_imp {p q : Nat → Prop} :
+    (∀ n, p n → q n) → (∃ n, ∀ m > n, p m) → (∃ n, ∀ m > n, q m) := by
+  intro imp ⟨n, fa⟩; refine ⟨n, λ m gt => imp m (fa m gt)⟩
+
+lemma fit_liftToExecution {evm : Devm}
+    {f : Except (String × State × AdrSet × Tra) Devm}
+    (fit : f.Fit) : (liftToExecution evm f).Fit := by
+  cases f
+  · exact fit
+  · simp only [liftToExecution]; intro ltd; cases ltd
+
+lemma ok_bind' {ξ υ ζ} {y : υ}
+    {f : υ → Except ξ ζ} {z : Except ξ ζ}
+    (eq : f y = z) : (.ok y >>= f) = z := by
+  rw [ok_bind]; exact eq
+
+syntax "efg_step_early " ident : tactic
+macro_rules
+  | `(tactic| efg_step_early $run) =>
+    `(tactic|
+      have temp := $run; clear $run;
+      rcases or_of_ite temp with ⟨pos, $run⟩ | ⟨neg, $run⟩ <;> clear temp <;> [
+        ( apply exists_forall_gt_imp (λ _ => ite_eq_left_of_true pos);
+          simp only [bind_pure]; clear pos );
+        ( apply exists_forall_gt_imp (λ _ => ite_eq_right_of_false neg ∘ ok_bind');
+          clear neg )
+      ]
+    )
+
+lemma of_generic_create' {sevm : Sevm} {devm : Devm} {endowment : B256} {newAddress : Adr}
+    {memoryIndex memorySize : ℕ} {xl : Xlot} {ex : Execution} (good : xl.Good')
+    (run : GenericCreate sevm devm endowment newAddress memoryIndex memorySize xl ex) :
+    ex.Fit ∧
+      ∃ lim,
+        ∀ lim' > lim,
+          genericCreate false sevm devm endowment
+            newAddress memoryIndex memorySize lim' = ex := by
+  simp only [GenericCreate] at run; constructor
+  · fit_step_exists run
+    fit_step_split run (fit_assert (by decide))
+    iterate 3 (fit_step_exists run);
+    fit_step_split run fit_assertDynamic
+    iterate 2 (fit_step_exists run);
+    split at run; {rw [← run]; apply fit_push}
+    fit_step_exists run
+    split at run; {rw [← run]; apply fit_push}
+    fit_step_exists run
+    fit_step_exec run good of_process_create_message' fit_liftToExecution
+    split at run <;> (rw [← run]; apply fit_push)
+  · apply Exists.imp forall_gt_of_forall_gt_succ_pred
+    simp only [genericCreate]
+    efg_step_exists run; efg_step_split run
+    iterate 3 (efg_step_exists run)
+    efg_step_split run; iterate 2 (efg_step_exists run)
+    efg_step_early run; {refine' ⟨0, _⟩; intro _ _; exact run}
+    efg_step_exists run
+    efg_step_early run; {refine' ⟨0, _⟩; intro _ _; exact run}
+    efg_step_exists run
+    efg_step_exec run good of_process_create_message'
+    eq_split run; eq_ite run <;> exact run
+
+lemma fit_map_rev {ξ υ ζ} {x : Except (String × ξ) υ}
+    {f : υ → ζ} : x.Fit → (x <&> f).Fit  := of_lim_map_rev.mt
+
+lemma of_generic_call' {sevm : Sevm} {devm : Devm} {gas : Nat} {value : B256}
+    {caller target codeAddress : Adr} {shouldTransferValue isStaticcall : Bool}
+    {input_index input_size output_index output_size : Nat} {code : ByteArray}
+    {disablePrecompiles : Bool} {xl : Xlot} {ex : Execution} (good : xl.Good')
+    ( run :
+      GenericCall sevm devm gas value caller target codeAddress
+        shouldTransferValue isStaticcall input_index input_size
+        output_index output_size code disablePrecompiles xl ex ) :
+    ex.Fit ∧
+      ∃ lim, ∀ lim' > lim,
+        genericCall false sevm devm gas value caller target codeAddress
+          shouldTransferValue isStaticcall input_index input_size
+          output_index output_size code disablePrecompiles lim' = ex := by
+  simp only [GenericCall] at run; constructor
+  · fit_step_exists run
+    split at run; {rw [← run]; apply fit_push}
+    fit_step_exists run
+    fit_step_exists run
+    fit_step_exec run good of_process_message' fit_liftToExecution
+    split at run <;>
+    {fit_step_split run fit_push; rw [← run]; apply fit_ok}
+  · apply Exists.imp forall_gt_of_forall_gt_succ_pred
+    simp only [genericCall]; efg_step_exists run;
+    efg_step_early run; {refine' ⟨0, _⟩; intro _ _; exact run}
+    efg_step_exists run; efg_step_exists run;
+    efg_step_exec run good of_process_message'; eq_split run;
+    eq_ite run <;> {eq_split run; exact run}
+
+syntax "efg_step_ite " ident : tactic
+macro_rules
+  | `(tactic| efg_step_ite $run) =>
+    `(tactic|
+      have temp := $run; clear $run;
+      rcases or_of_ite temp with ⟨pos, $run⟩ | ⟨neg, $run⟩ <;> clear temp <;> [
+        ( apply exists_forall_gt_imp (λ _ => ite_eq_left_of_true pos);
+
+          clear pos );
+        ( apply exists_forall_gt_imp (λ _ => ite_eq_right_of_false neg);
+          clear neg )
+      ]
+    )
+
+lemma Ninst.run_of_run' {pc} {sevm} {devm} {n : Ninst} (xl : Xlot)
+    {ex} (good : xl.Good') (run : Ninst.Run' pc sevm devm n xl ex) :
+    ex.Fit ∧ ∃ lim, ∀ lim' > lim, Ninst.run false ⟨pc, sevm, devm⟩ n lim' = ex := by
+  rcases n with r | x | ⟨xs, le⟩
+  · simp only [Ninst.Run'] at run
+    simp only [Ninst.run]; constructor;
+    · rw [← run]; apply fit_withPc Rinst.fit_run
+    · refine ⟨0, λ _ _ => run⟩;
+  · cases x <;>
+      ( constructor <;>
+        [ skip;
+          (apply Exists.imp forall_gt_of_forall_gt_succ_pred ; simp only [Ninst.run]) ] )
+    · fit_step_split run fit_pop
+      fit_step_split run fit_popToNat
+      fit_step_split run fit_popToNat
+      fit_step_exists run; fit_step_exists run
+      fit_step_split run fit_chargeGas
+      fit_step_exists run; fit_step_exists run
+      fit_step_exec run good of_generic_create' id
+      rw [← run]; apply fit_ok
+    · iterate 3 (efg_step_split run)
+      efg_step_exists run; efg_step_exists run
+      efg_step_split run
+      efg_step_exists run; efg_step_exists run
+      efg_step_exec run good of_generic_create'
+      eq_split run; exact run
+    · fit_step_split run fit_pop
+      fit_step_split run (fit_map_rev fit_pop)
+      fit_step_split run fit_pop
+      iterate 4 (fit_step_split run fit_popToNat)
+      iterate 3 (fit_step_exists run)
+      fit_step_exists run
+      iterate 3 (fit_step_exists run)
+      fit_step_exists run
+      fit_step_split run fit_chargeGas
+      fit_step_split run (fit_assert (by decide))
+      fit_step_exists run; fit_step_exists run
+      split at run
+      · fit_step_split run fit_push
+        rw [← run]; apply fit_ok
+      · fit_step_exec run good of_generic_call' id
+        rw [← run]; apply fit_ok
+    · iterate 7 (efg_step_split run)
+      iterate 3 (efg_step_exists run)
+      efg_step_exists run;
+      iterate 3 (efg_step_exists run)
+      efg_step_exists run;
+      efg_step_split run; efg_step_split run;
+      efg_step_exists run; efg_step_exists run;
+      efg_step_ite run
+      · efg_step_split run; refine ⟨0, λ _ _ => run⟩
+      · efg_step_exec run good of_generic_call'
+        eq_split run; exact run
+    · fit_step_split run fit_pop
+      fit_step_split run (fit_map_rev fit_pop)
+      fit_step_split run fit_pop
+      iterate 4 (fit_step_split run fit_popToNat)
+      iterate 4 (fit_step_exists run)
+      fit_step_exists run
+      fit_step_exists run; fit_step_exists run
+      fit_step_split run fit_chargeGas
+      fit_step_exists run; fit_step_exists run
+      split at run
+      · fit_step_split run fit_push
+        rw [← run]; apply fit_ok
+      · fit_step_exec run good of_generic_call' id
+        rw [← run]; apply fit_ok
+    · iterate 7 (efg_step_split run)
+      iterate 3 (efg_step_exists run)
+      efg_step_exists run;
+      iterate 2 (efg_step_exists run)
+      efg_step_exists run;
+      efg_step_split run
+      iterate 2 (efg_step_exists run)
+      efg_step_ite run
+      · efg_step_split run; refine ⟨0, λ _ _ => run⟩
+      · efg_step_exec run good of_generic_call'
+        eq_split run; exact run
+    · fit_step_split run fit_pop
+      fit_step_split run (fit_map_rev fit_pop)
+      iterate 4 (fit_step_split run fit_popToNat)
+      iterate 3 (fit_step_exists run)
+      fit_step_exists run
+      fit_step_exists run
+      fit_step_exists run
+      fit_step_split run fit_chargeGas
+      fit_step_exists run;
+      fit_step_exec run good of_generic_call' id
+      rw [← run]; apply fit_ok
+    · iterate 6 (efg_step_split run)
+      iterate 3 (efg_step_exists run)
+      efg_step_exists run;
+      efg_step_exists run
+      efg_step_exists run;
+      efg_step_split run
+      efg_step_exists run
+      efg_step_exec run good of_generic_call'
+      eq_split run; exact run
+    · fit_step_split run fit_pop
+      iterate 2 (fit_step_split run fit_popToNat)
+      fit_step_split run fit_pop
+      iterate 3 (fit_step_exists run)
+      fit_step_split run fit_chargeGas
+      iterate 2 (fit_step_exists run)
+      fit_step_exec run good of_generic_create' id
+      rw [← run]; apply fit_ok
+    · iterate 4 (efg_step_split run)
+      iterate 3 (efg_step_exists run)
+      efg_step_split run
+      iterate 2 (efg_step_exists run)
+      efg_step_exec run good of_generic_create'
+      eq_split run; exact run
+    · fit_step_split run fit_pop
+      fit_step_split run (fit_map_rev fit_pop)
+      iterate 4 (fit_step_split run fit_popToNat)
+      iterate 3 (fit_step_exists run)
+      fit_step_exists run
+      fit_step_exists run
+      fit_step_exists run
+      fit_step_split run fit_chargeGas
+      fit_step_exists run;
+      fit_step_exec run good of_generic_call' id
+      rw [← run]; apply fit_ok
+    · iterate 6 (efg_step_split run)
+      iterate 3 (efg_step_exists run)
+      efg_step_exists run;
+      efg_step_exists run
+      efg_step_exists run;
+      efg_step_split run
+      efg_step_exists run
+      efg_step_exec run good of_generic_call'
+      eq_split run; exact run
+  · simp [Ninst.Run'] at run; constructor
+    · rw [← run]; intro ltd
+      fit_bind_step ltd fit_chargeGas
+      fit_bind_step ltd fit_push; cases ltd
+    · simp only [Ninst.run]; refine' ⟨0, λ _ _ => run⟩
+
+lemma Except.bind_eq_of_is_error {ξ υ : Type} {e : Except ξ υ}
+    {f : υ → Except ξ υ} : e.IsError → (e >>= f) = e := by
+  intro h; cases e
+  · rfl
+  · cases h
+
+lemma Jinst.fit_run {evm} {j : Jinst} : (Jinst.run evm j).Fit := by
+  intro ltd; cases j <;> simp only [Jinst.run] at ltd
+  case jumpi =>
+    fit_bind_step ltd fit_pop
+    fit_bind_step ltd fit_pop
+    fit_bind_step ltd fit_chargeGas
+    split at ltd
+    · fit_bind_step ltd fit_ok; cases ltd
+    · fit_bind_step ltd (fit_assert (by decide))
+      fit_bind_step ltd fit_ok; cases ltd
+  case jumpdest =>
+    fit_bind_step ltd fit_chargeGas; cases ltd
+  case jump =>
+    fit_bind_step ltd fit_pop
+    fit_bind_step ltd fit_chargeGas
+    fit_bind_step ltd (fit_assert (by decide))
+    cases ltd
+
+lemma Linst.fit_run {sevm} {devm} {l : Linst} : (Linst.run sevm devm l).Fit := by
+  intro ltd; cases l
+  case stop => cases ltd
+  case rev =>
+    fit_bind_step ltd fit_popToNat
+    fit_bind_step ltd fit_popToNat
+    fit_bind_step ltd fit_chargeGas
+    simp [Except.Lim, Except.toError?] at ltd
+  case ret =>
+    fit_bind_step ltd fit_popToNat
+    fit_bind_step ltd fit_popToNat
+    fit_bind_step ltd fit_chargeGas
+    simp [Except.Lim, Except.toError?] at ltd
+  case dest =>
+    simp only [Devm.popToAdr, bind_map_left, Linst.run] at ltd
+    fit_bind_step ltd fit_pop
+    fit_bind_step ltd fit_chargeGas
+    fit_bind_step ltd fit_assertDynamic
+    have ne : "ERROR : InsufficientBalanceError" ≠ "RecursionLimit" := by decide
+    fit_bind_step ltd (fit_to_except ne)
+    split at ltd <;> simp [Except.Lim, Except.toError?] at ltd
+
+lemma of_exec' :
+    ∀ (pc : Nat) (sevm : Sevm) (devm : Devm) (exn : Execution),
+      Exec pc sevm devm exn →
+      exn.Fit ∧
+        ∃ lim, ∀ lim' > lim, (exec false ⟨pc, sevm, devm⟩ lim' = exn) := by
+  apply Exec.rec
+  · intro pc sevm devm eq; refine' ⟨_, 0, _⟩
+    · intro ltd; injection ltd; contradiction
+    · intro lim' gt; cases lim'; {cases Nat.not_lt_zero _ gt}
+      simp only [exec, Option.toExcept, Evm.getInst, eq]; rfl
+  · intro pc sevm devm n err devm' nat run
+    rcases Ninst.run_of_run' .none .intro run with ⟨fit, lim, eq⟩
+    refine' ⟨fit, lim + 2, _⟩
+    intro lim' gt; rcases lim' with _ | lim'; {cases Nat.not_lt_zero _ gt}
+    simp only [Ninst.At] at nat
+    simp only [Evm.getInst, exec, Option.toExcept, nat, ok_bind]
+    rw [eq lim' (by omega)]; rfl
+  · intro pc sevm devm n evm' exn' exn devm' nat run exc ⟨fit', limExec, exec_eq⟩
+    rcases
+      Ninst.run_of_run'
+        (.some ⟨evm', exn'⟩)
+        ⟨fit', limExec + 1, exec_eq _ (by omega)⟩
+        run
+      with ⟨fit, limRun, run_eq⟩
+    refine' ⟨fit, (max limExec limRun) + 1, _⟩
+    intro lim' gt; rcases lim' with _ | lim'; {cases Nat.not_lt_zero _ gt}
+    simp only [Ninst.At] at nat
+    simp only [Evm.getInst, ok_bind, exec, Option.toExcept, nat]
+    rw [run_eq lim' (by omega)]; rfl
+  · intro pc sevm devm n pc' devm' exn nat run exc ⟨fit, limExec, exec_eq⟩
+    rcases Ninst.run_of_run' .none .intro run
+      with ⟨temp, limRun, run_eq⟩; clear temp
+    refine' ⟨fit, (max limExec limRun) + 1, _⟩
+    intro lim' gt; rcases lim' with _ | lim'; {cases Nat.not_lt_zero _ gt}
+    simp only [Ninst.At] at nat
+    simp only [Evm.getInst, ok_bind, exec, Option.toExcept, nat]
+    rw [run_eq lim' (by omega)]; apply exec_eq _ (by omega)
+  · intro pc devm devm n evm' exn' pc'' devm'' exn nat run exc' exc
+      ⟨fit', limExec', exec_eq'⟩
+      ⟨fit, limExec, exec_eq⟩
+    rcases
+      Ninst.run_of_run'
+        (.some ⟨evm', exn'⟩)
+        ⟨fit', limExec' + 1, exec_eq' _ (by omega)⟩
+        run
+      with ⟨fitRun, limRun, run_eq⟩
+    refine' ⟨fit, max limRun limExec + 1, _⟩
+    intro lim' gt; rcases lim' with _ | lim'; {cases Nat.not_lt_zero _ gt}
+    simp only [Ninst.At] at nat
+    simp only [Evm.getInst, ok_bind, _root_.exec, Option.toExcept, nat]
+    rw [run_eq lim' (by omega)]
+    apply exec_eq _ (by omega)
+  · intro pc sevm devm j err devm' nat run
+    simp only [Jinst.At] at nat
+    simp only [Jinst.Run] at run
+    constructor
+    · have fit := @Jinst.fit_run ⟨pc, sevm, devm⟩ j
+      rw [run] at fit; exact fit
+    · refine' ⟨0, _⟩; intro lim gt
+      rcases lim with _ | lim; {cases Nat.not_lt_zero _ gt}
+      simp only [Evm.getInst, exec, nat, Option.toExcept, ok_bind, run]; rfl
+  · intro pc sevm devm j pc' devm' exn jat run exc ⟨fit, lim, exec_eq⟩
+    simp only [Jinst.At] at jat
+    simp only [Jinst.Run] at run
+    refine' ⟨fit, lim + 1, _⟩; intro lim' gt
+    rcases lim' with _ | lim'; {cases Nat.not_lt_zero _ gt}
+    simp only [Evm.getInst, exec, jat, Option.toExcept, ok_bind, run]
+    apply exec_eq _ (by omega)
+  · intro pc sevm devm l exn lat run
+    simp only [Linst.At] at lat
+    simp only [Linst.Run] at run
+    have fit := @Linst.fit_run sevm devm l; rw [run] at fit
+    refine' ⟨fit, 0, _⟩; intro lim' gt
+    rcases lim' with _ | lim'; {cases Nat.not_lt_zero _ gt}
+    simp only [Evm.getInst, exec, lat, Option.toExcept, ok_bind, run]
+
+def Xlot.Good (lim : Nat) (oe : Option String) : Xlot → Prop
+  | .none => True
+  | .some (evm, ex) =>
+    ∃ lim' < lim,
+      exec false evm lim' = ex ∧
+      (ex.toError? = some "RecursionLimit" → oe = some "RecursionLimit")
+
+syntax "bind_step_good " ident rcasesPat : tactic
+macro_rules
+  | `(tactic| bind_step_good $h $pat) => `(tactic|
+      rcases of_bind_eq $h with im | ⟨$pat, temp_eq, eq'⟩;
+      { refine ⟨.none, .intro, .inl im⟩ };
+      clear $h; rename' eq' => $h;
+      apply Exists.imp
+        (λ _ (conj : _ ∧ _) => ⟨conj.1, Or.inr ⟨_, temp_eq, conj.2⟩⟩);
+      clear temp_eq
+    )
+
+syntax "okStep1 " ident rcasesPat : tactic
+macro_rules
+  | `(tactic| okStep1 $h $pat1) => `(tactic|
+      rcases of_bind_eq $h with ⟨_, ⟨_⟩, _⟩ | ⟨$pat1, temp_eq, eq'⟩;
+      clear $h; rename' eq' => $h;
+      apply Exists.imp
+        (λ _ (conj : _ ∧ _) => ⟨conj.1, ⟨_, (Except.ok.inj temp_eq).symm, conj.2⟩⟩);
+      clear temp_eq
+    )
+
+syntax "okStep2 " ident rcasesPat rcasesPat : tactic
+macro_rules
+  | `(tactic| okStep2 $h $pat1 $pat2) => `(tactic|
+      rcases of_bind_eq $h with ⟨_, ⟨_⟩, _⟩ | ⟨⟨$pat1, $pat2⟩, temp_eq, eq'⟩;
+      clear $h; rename' eq' => $h;
+      apply Exists.imp
+        (λ _ (conj : _ ∧ _) => ⟨conj.1, ⟨_, (Except.ok.inj temp_eq).symm, conj.2⟩⟩);
+      clear temp_eq
+    )
+
+syntax "okStep5 " ident rcasesPat rcasesPat rcasesPat rcasesPat rcasesPat : tactic
+macro_rules
+  | `(tactic| okStep5 $h $pat1 $pat2 $pat3 $pat4 $pat5) => `(tactic|
+      rcases of_bind_eq $h
+        with ⟨_, ⟨_⟩, _⟩ | ⟨⟨$pat1, $pat2, $pat3, $pat4, $pat5⟩, temp_eq, eq'⟩;
+      clear $h; rename' eq' => $h;
+      apply Exists.imp
+        (λ _ (conj : _ ∧ _) => ⟨conj.1, ⟨_, (Except.ok.inj temp_eq).symm, conj.2⟩⟩);
+      clear temp_eq
+    )
+
+syntax "bind_step' " ident rcasesPat : tactic
+macro_rules
+  | `(tactic| bind_step' $h $pat) => `(tactic|
+      rcases of_bind_eq $h with im | ⟨$pat, temp_eq, eq'⟩;
+      {left; exact im}; clear $h; rename' eq' => $h;
+      right; refine' ⟨_, temp_eq, _⟩; clear temp_eq
+    )
+
+lemma Except.fit_of_fit {ξ} {υ} {ζ}
+    {f : Except (String × ξ) υ}
+    {g : υ → Except (String × ξ) ζ}
+    {ex : Except (String × ξ) ζ}
+    (notLimited : ex.Fit) (eq : f >>= g = ex) : f.Fit := by
+  intro rw; rcases f with ⟨_, _⟩ | _ <;>
+    simp [Except.Lim, Except.toError?] at rw
+  rw [rw] at eq; rw [← eq] at notLimited; cases notLimited rfl
+
+lemma Execution.fit_of_fit {ξ} {υ}
+    {f : Except (String × Devm) ξ}
+    {g : ξ → Except (String × Devm) υ}
+    {ex : Except (String × Devm) υ}
+    (fit : ex.Fit) (eq : f >>= g = ex) : f.Fit := by
+  intro rw; rcases f with ⟨evm, err⟩ | _ <;>
+    simp [Except.Lim, Except.toError?] at rw
+  rw [rw] at eq; rw [← eq] at fit; cases fit rfl
+
+lemma ite_of_true {c : Prop} [Decidable c] {p q : Prop} :
+    c → p → if c then p else q := by
+  intro hc hp; rw [if_pos hc]; exact hp
+
+lemma ite_of_false {c : Prop} [Decidable c] {p q : Prop} :
+    ¬ c → q → if c then p else q := by
+  intro hc hp; rw [if_neg hc]; exact hp
+
+lemma Except.of_toError?_eq_some {ξ} {υ} (ex : Except (String × ξ) υ)
+    (err : String) (eq : ex.toError? = some err) :
+    ∃ x, ex = .error ⟨err, x⟩ := by
+  rcases ex with ⟨err', _⟩ | _ <;> simp [Except.toError?] at eq
+  cases eq; refine ⟨_, rfl⟩
+
+lemma of_executeCode {msg : Msg} {lim : Nat}
+    {ex : Except (String × State × AdrSet × Tra) Devm}
+    (notLimited : ex.toError? ≠ some "RecursionLimit")
+    (eq : executeCode false msg lim = ex) :
+    ∃ xl : Xlot, xl.Good lim ex.toError? ∧ ExecuteCode msg xl ex := by
+  rcases lim with _ | lim <;> simp only [executeCode] at eq
+  {rw [← eq] at notLimited; cases notLimited rfl}
+  split at eq
+  · rename msg.codeAddress = .none => eq_none
+    refine'
+      ⟨ .some ⟨initEvm msg, exec false (initEvm msg) lim⟩,
+        ⟨lim, (by omega), rfl, λ halts => _⟩, _ ⟩
+    · rcases Except.of_toError?_eq_some _ _ halts with ⟨evm, rw⟩
+      rw [← eq, rw] at notLimited; cases notLimited rfl
+    · simp only [ExecuteCode]; rw [eq_none]; refine' ⟨_, rfl, eq⟩
+  · rename Adr => adr
+    rename msg.codeAddress = .some adr => eq_some
+    split at eq
+    · rename_i pos; refine' ⟨.none, .intro, _⟩
+      simp only [ExecuteCode]; rw [eq_some]
+      simp only []; rw [if_pos pos]; simp [eq]
+    · rename_i neg
+      refine'
+        ⟨ .some ⟨initEvm msg, exec false (initEvm msg) lim⟩,
+          ⟨lim, (by omega), rfl, λ halts => _⟩, _ ⟩
+      · rcases Except.of_toError?_eq_some _ _ halts with ⟨evm, rw⟩
+        rw [← eq, rw] at notLimited; cases notLimited rfl
+      · simp only [ExecuteCode]; rw [eq_some]
+        simp only []; rw [if_neg neg]; refine' ⟨_, rfl, eq⟩
+
+lemma Xlot.good_of_good_of_notLimited {lim lim' : Nat} {oe oe' : Option String}
+    {xl : Xlot} (le : lim ≤ lim') (ne : oe ≠ some "RecursionLimit")
+    (good : xl.Good lim oe) : xl.Good lim' oe' := by
+  rcases xl with _ | ⟨evm, ex⟩; {constructor}
+  rcases good with ⟨_, lt, exec, of_eq⟩
+  refine' ⟨_, Nat.lt_of_lt_of_le lt le, exec,  _⟩
+  intro eq; cases ne <| of_eq eq
+
+lemma of_processMessage (msg : Msg) (lim : Nat)
+    (ex : Except (String × State × AdrSet × Tra) Devm)
+    (notLimited : ex.toError? ≠ some "RecursionLimit")
+    (eq : processMessage false msg lim = ex) :
+    ∃ xl : Xlot, xl.Good lim ex.toError? ∧ ProcessMessage msg xl ex := by
+  rcases lim with _ | lim <;> simp only [processMessage] at eq
+  {rw [← eq] at notLimited; cases notLimited rfl}
+  bind_step_good eq _; bind_step_good eq _
+  have notLimited' := Except.fit_of_fit notLimited eq
+  rcases of_executeCode notLimited' rfl with ⟨xl, good, ec⟩
+  refine' ⟨_, Xlot.good_of_good_of_notLimited (by omega) notLimited' good, _, ec, _⟩
+  bind_step' eq _; split at eq
+  · rename_i pos; rw [if_pos pos]; exact eq
+  · rename_i neg; rw [if_neg neg]; exact eq
+
+lemma of_processCreateMessage (msg : Msg) (lim : Nat)
+    (ex : Except (String × State × AdrSet × Tra) Devm)
+    (notLimited : ex.toError? ≠ some "RecursionLimit")
+    (eq : processCreateMessage false msg lim = ex) :
+    ∃ xl : Xlot,
+      xl.Good lim ex.toError? ∧
+      ProcessCreateMessage msg xl ex := by
+  rcases lim with _ | lim <;> simp only [processCreateMessage] at eq
+  {rw [← eq] at notLimited; cases notLimited rfl}
+  have notLimited' :
+    (processMessage false (processCreateMessage.msg msg) lim).toError?
+      ≠ some "RecursionLimit" := by
+    intro pm_eq
+    rcases Except.of_toError?_eq_some _ _ pm_eq with ⟨_, rw⟩
+    rw [← eq, rw] at notLimited
+    cases notLimited rfl
+  rcases @of_processMessage _ _ _ notLimited' rfl
+    with ⟨xl, good, pcm⟩
+  refine' ⟨_, Xlot.good_of_good_of_notLimited (by omega) notLimited' good, _, pcm, _⟩
+  bind_step' eq evm'
+  split at eq
+  · rename_i pos; rw [if_pos pos]
+    cases pcm_eq : processCreateMessage.chargeCodeGas evm'
+    · simp only []
+      rw [pcm_eq] at eq
+      simp only [] at eq
+      split at eq
+      · rename_i pos; rw [if_pos pos]; exact eq
+      · rename_i neg; rw [if_neg neg]; exact eq
+    · rw [pcm_eq] at eq; exact eq
+  · rename_i neg; rw [if_neg neg]; exact eq
+
+lemma of_genericCreate
+    {sevm : Sevm} {devm : Devm} {endow : B256} {newAdr : Adr}
+    {memIndex memSize lim : ℕ} {ex : Execution}
+    (notLimited : ex.toError? ≠ some "RecursionLimit")
+    (eq : genericCreate false sevm devm endow newAdr memIndex memSize lim = ex) :
+    ∃ xl : Xlot,
+      xl.Good lim ex.toError? ∧
+      GenericCreate sevm devm endow newAdr memIndex memSize xl ex := by
+  rcases lim with _ | lim <;> simp only [genericCreate] at eq
+  {rw [← eq] at notLimited; cases notLimited rfl}
+  okStep1 eq _; bind_step_good eq _; okStep1 eq _; okStep1 eq _
+  okStep1 eq _; bind_step_good eq _; okStep1 eq _; okStep1 eq _
+  split at eq
+  · rename_i pos
+    apply Exists.imp (λ _ (conj : _ ∧ _) => ⟨conj.1, ite_of_true pos conj.2⟩)
+    rcases of_bind_eq eq with ⟨es, push_eq, ex_eq⟩ | ⟨evm, push_eq, eq_ex⟩;
+    · refine' ⟨.none, .intro, _⟩; rw [ex_eq]; exact push_eq
+    · refine' ⟨.none, .intro, _⟩; rw [← eq_ex]; exact push_eq
+  · rename_i neg
+    apply Exists.imp (λ _ (conj : _ ∧ _) => ⟨conj.1, ite_of_false neg conj.2⟩)
+    clear neg; simp at eq
+    okStep1 eq evm'
+    split at eq
+    · rename_i pos
+      apply Exists.imp (λ _ (conj : _ ∧ _) => ⟨conj.1, ite_of_true pos conj.2⟩)
+      refine' ⟨.none, .intro, eq⟩
+    · rename_i neg
+      apply Exists.imp (λ _ (conj : _ ∧ _) => ⟨conj.1, ite_of_false neg conj.2⟩)
+      clear neg
+      okStep1 eq msg
+      have notLimited' :
+          (processCreateMessage false msg lim).toError?
+            ≠ some "RecursionLimit" := by
+        intro pm_eq
+        rcases Except.of_toError?_eq_some _ _ pm_eq with ⟨_, rw⟩
+        rw [← eq, rw] at notLimited; cases notLimited rfl
+      rcases of_processCreateMessage _ _ _ notLimited' rfl
+        with ⟨xl, good, pm⟩
+      refine' ⟨_, Xlot.good_of_good_of_notLimited (by omega) notLimited' good, _, pm, _⟩
+      bind_step' eq _
+      split at eq
+      · rename_i pos; rw [if_pos pos]; exact eq
+      · rename_i neg; rw [if_neg neg]; exact eq
+
+lemma of_genericCall {sevm : Sevm} {devm : Devm} {gas : Nat} {value : B256}
+    {caller target codeAddress : Adr} {shouldTransferValue isStaticcall : Bool}
+    {input_index input_size output_index output_size : Nat} {code : ByteArray}
+    {disablePrecompiles : Bool} {lim : Nat} {ex : Execution}
+    (notLimited : ex.Fit)
+    ( eq :
+      genericCall false sevm devm gas value caller target codeAddress
+        shouldTransferValue isStaticcall input_index input_size
+        output_index output_size code disablePrecompiles lim = ex ) :
+    ∃ xl : Xlot,
+      xl.Good lim ex.toError? ∧
+      GenericCall sevm devm gas value caller target codeAddress
+        shouldTransferValue isStaticcall input_index input_size
+        output_index output_size code disablePrecompiles xl ex := by
+  rcases lim with _ | lim <;> simp only [genericCall] at eq
+  {rw [← eq] at notLimited; cases notLimited rfl}
+  okStep1 eq _; split at eq
+  { rename_i pos; refine' ⟨.none, .intro, _⟩
+    simp only [bind_pure] at eq;
+    simp only []; rw [if_pos pos, eq] }
+  rename_i neg
+  apply Exists.imp (λ _ (h' : _ ∧ _) => ⟨h'.1, ite_of_false neg h'.2⟩);
+  simp only [pure_bind] at eq
+  okStep1 eq _; okStep1 eq msg
+  have notLimited' :
+    (processMessage false msg lim).toError? ≠ some "RecursionLimit" := by
+    intro pm_eq
+    rcases Except.of_toError?_eq_some _ _ pm_eq with ⟨_, rw⟩
+    rw [← eq, rw] at notLimited
+    cases notLimited rfl
+  rcases of_processMessage msg lim _ notLimited' rfl
+    with ⟨xl, good, pm⟩
+  refine' ⟨_, Xlot.good_of_good_of_notLimited (by omega) notLimited' good, _, pm, _⟩
+  bind_step' eq _
+  split at eq
+  · rename_i pos; rw [if_pos pos]; bind_step' eq _; exact eq
+  · rename_i neg; rw [if_neg neg]; bind_step' eq _; exact eq
+
+lemma Ninst.run_of_run
+    {pc}
+    {sevm : Sevm}
+    {devm : Devm}
+    {n : Ninst} {lim : Nat}
+    {exn} (notLimited : exn.Fit)
+    (eq : Ninst.run false ⟨pc, sevm, devm⟩ n lim = exn) :
+    ∃ xl : Xlot,
+      xl.Good lim exn.toError? ∧
+      Ninst.Run' pc sevm devm n xl exn :=
+  match n, lim with
+  | exec _, 0 => by
+    simp only [Ninst.run] at eq
+    rw [← eq] at notLimited
+    cases notLimited rfl
+  | push xs lt, lim => by
+    refine' ⟨.none, .intro, _⟩
+    simp only [Ninst.run] at eq; apply eq
+  | reg r, _ => by
+    simp [Ninst.run] at eq
+    refine' ⟨.none, .intro, eq⟩
+  | exec .create, lim + 1 => by
+    simp only [Ninst.run] at eq
+    bind_step_good eq _
+    bind_step_good eq _; bind_step_good eq _; okStep1 eq _;
+    okStep1 eq _; bind_step_good eq _; okStep1 eq _; okStep1 eq _;
+    have notLimited' := Execution.fit_of_fit notLimited eq
+    rcases of_genericCreate notLimited' rfl with ⟨xl, good, gc⟩
+    refine' ⟨_, Xlot.good_of_good_of_notLimited (by omega) notLimited' good, _, gc, _⟩
+    bind_step' eq _; exact eq;
+  | exec .create2, lim + 1 => by
+    simp only [Ninst.run] at eq
+    bind_step_good eq _; bind_step_good eq _; bind_step_good eq _;
+    bind_step_good eq _; okStep1 eq _; okStep1 eq _; okStep1 eq _;
+    bind_step_good eq _; okStep1 eq _; okStep1 eq _;
+    have notLimited' := Execution.fit_of_fit notLimited eq
+    rcases of_genericCreate notLimited' rfl with ⟨xl, good, gc⟩
+    refine' ⟨_, Xlot.good_of_good_of_notLimited (by omega) notLimited' good, _, gc, _⟩
+    bind_step' eq _; exact eq
+  | exec .call, lim + 1 => by
+    simp only [Ninst.run] at eq
+    bind_step_good eq _; bind_step_good eq _; bind_step_good eq _;
+    bind_step_good eq _; bind_step_good eq _; bind_step_good eq _;
+    bind_step_good eq _; okStep1 eq _; okStep1 eq _; okStep1 eq _;
+    okStep5 eq _ _ _ _ _; okStep1 eq _; okStep1 eq _; okStep1 eq _;
+    okStep2 eq _ _; bind_step_good eq _; bind_step_good eq _;
+    okStep1 eq _; okStep1 eq _; split at eq
+    · rename_i lt
+      refine' ⟨.none, .intro, _⟩
+      simp only []
+      rw [if_pos lt]
+      bind_step' eq _; exact eq
+    · rename_i nlt
+      apply Exists.imp (λ _ (conj : _ ∧ _) => ⟨conj.1, ite_of_false nlt conj.2⟩)
+      have notLimited' := Execution.fit_of_fit notLimited eq
+      rcases of_genericCall notLimited' rfl with ⟨xl, good, gc⟩
+      refine' ⟨_, Xlot.good_of_good_of_notLimited (by omega) notLimited' good, _, gc, _⟩
+      bind_step' eq _; exact eq
+  | exec .callcode, lim + 1 => by
+    simp only [Ninst.run] at eq
+    bind_step_good eq _; bind_step_good eq _; bind_step_good eq _;
+    bind_step_good eq _; bind_step_good eq _; bind_step_good eq _;
+    bind_step_good eq _; okStep1 eq _; okStep1 eq _;
+    okStep1 eq _; okStep5 eq _ _ _ _ _; okStep1 eq _; okStep1 eq _;
+    okStep2 eq _ _; bind_step_good eq _; okStep1 eq _; okStep1 eq _;
+    split at eq
+    · rename_i lt; refine' ⟨.none, .intro, _⟩
+      simp only []
+      rw [if_pos lt]; bind_step' eq _; exact eq
+    · rename_i nlt
+      apply Exists.imp (λ _ (conj : _ ∧ _) => ⟨conj.1, ite_of_false nlt conj.2⟩)
+      have notLimited' := Execution.fit_of_fit notLimited eq
+      rcases of_genericCall notLimited' rfl with ⟨xl, good, gc⟩
+      refine' ⟨_, Xlot.good_of_good_of_notLimited (by omega) notLimited' good, _, gc, _⟩
+      bind_step' eq _; exact eq
+  | exec .delcall, lim + 1 => by
+    simp only [Ninst.run] at eq
+    bind_step_good eq _; bind_step_good eq _; bind_step_good eq _;
+    bind_step_good eq _; bind_step_good eq _; bind_step_good eq _;
+    okStep1 eq _; okStep1 eq _; okStep1 eq _; okStep5 eq _ _ _ _ _;
+    okStep1 eq _; okStep2 eq _ _; bind_step_good eq _; okStep1 eq _;
+    have notLimited' := Execution.fit_of_fit notLimited eq
+    rcases of_genericCall notLimited' rfl with ⟨xl, good, gc⟩
+    refine' ⟨_, Xlot.good_of_good_of_notLimited (by omega) notLimited' good, _, gc, _⟩
+    bind_step' eq _; exact eq
+  | exec .statcall, lim + 1 => by
+    simp only [Ninst.run] at eq
+    bind_step_good eq _; bind_step_good eq _; bind_step_good eq _;
+    bind_step_good eq _; bind_step_good eq _; bind_step_good eq _;
+    okStep1 eq _; okStep1 eq _; okStep1 eq _; okStep5 eq _ _ _ _ _;
+    okStep1 eq _; okStep2 eq _ _; bind_step_good eq _; okStep1 eq _;
+    have notLimited' := Execution.fit_of_fit notLimited eq
+    rcases of_genericCall notLimited' rfl with ⟨xl, good, gc⟩
+    refine' ⟨_, Xlot.good_of_good_of_notLimited (by omega) notLimited' good, _, gc, _⟩
+    bind_step' eq _; exact eq
+
+def of_exec :
+    ∀ (lim : Nat) (pc : Nat) (sevm : Sevm) (devm : Devm) (exn : Execution),
+      exn.Fit → (exec false ⟨pc, sevm, devm⟩ lim = exn) →
+      Nonempty (Exec pc sevm devm exn) := by
+  apply Nat.strongRec; intro lim ih pc sevm devm exn fit exec_eq;
+  cases lim with
+  | zero =>
+    rw [← exec_eq] at fit
+    simp [exec, Except.toError?, Except.Fit, Except.Lim] at fit
+  | succ lim =>
+    simp [exec] at exec_eq
+    rcases Option.eq_none_or_eq_some (Evm.getInst ⟨pc, sevm, devm⟩) with
+      getInst_eq | ⟨i, getInst_eq⟩
+      <;> rw [getInst_eq] at exec_eq
+      <;> simp [Option.toExcept] at exec_eq
+    · rw [← Except.of_error_bind_eq _ exec_eq]
+      constructor; apply Exec.invOp getInst_eq
+    · rw [ok_bind] at exec_eq
+      rcases i with l | n | j <;> simp only [] at exec_eq
+      · constructor;
+        apply Exec.last getInst_eq exec_eq
+      · rcases of_bind_eq exec_eq with
+          ⟨es, run_eq, ex_eq⟩ | ⟨evm', run_eq, ex_eq⟩
+        · rw [ex_eq] at fit
+          rcases Ninst.run_of_run fit run_eq
+            with ⟨_ | ⟨evm', ex'⟩, good, run⟩
+          · rw [ex_eq]; constructor
+            exact Exec.nextNoneErr getInst_eq run
+          · rw [ex_eq];
+            have ne_ex : Nonempty (Exec evm'.pc evm'.sta evm'.dyna ex') := by
+              rcases good with ⟨lim', lt, exec_eq', notLimited_of⟩
+              have fit' : ex'.Fit := by
+                intro h; cases fit <| notLimited_of h
+              apply @ih _ (by omega) _ _ _ _ fit' exec_eq'
+            rcases ne_ex with ⟨exc⟩; constructor
+            apply Exec.nextSomeErr getInst_eq run exc
+        · rcases Ninst.run_of_run (by {intro h; cases h}) run_eq
+            with ⟨_ | ⟨evm', ex'⟩, good, run⟩
+          · rcases (ih _ (by omega) _ _ _ _ fit ex_eq) with ⟨exc⟩
+            constructor
+            exact @Exec.nextNoneRec _ _ _ _ _ _ _ getInst_eq run exc
+          · rcases good with ⟨lim', lt, exec_eq', notLimited_of⟩
+            have fit' : ex'.Fit := by intro h; cases notLimited_of h
+            rcases @ih _ (by omega) _ _ _ _ fit' exec_eq' with ⟨ih'⟩
+            rcases @ih _ (by omega) _ _ _ _ fit ex_eq with ⟨ih''⟩
+            constructor
+            apply @Exec.nextSomeRec _ _ _ _ _ _ _ _ _ getInst_eq run ih' ih''
+      · rcases of_bind_eq exec_eq
+          with ⟨es, run_eq, ex_eq⟩ | ⟨evm', run_eq, ex_eq⟩
+        · rw [ex_eq]; constructor
+          exact @Exec.jumpErr pc sevm devm j es.1 es.2 getInst_eq run_eq
+        · rcases ih _ (Nat.lt_succ_self _) _ _ _ _ fit ex_eq with ⟨ih'⟩
+          constructor; apply Exec.jumpRec getInst_eq run_eq ih'
+
+lemma exec_iff_exec (pc : Nat) (sevm : Sevm) (devm : Devm) (exn : Execution) :
+    Nonempty (Exec pc sevm devm exn) ↔
+      (exn.Fit ∧ ∃ lim, exec false ⟨pc, sevm, devm⟩ lim = exn) := by
+  constructor
+  · intro ⟨exc⟩;
+    rcases of_exec' _ _ _ _ exc with ⟨fit, lim, eq⟩
+    refine ⟨fit, lim + 1, eq (lim + 1) (by omega)⟩
+  · intro ⟨fit, lim, eq⟩; exact of_exec _ _ _ _ _ fit eq
